format-version: 1.2
date: 10:03:2024 17:10
saved-by: Lukas_Mueller
default-namespace: INV
ontology: CO_365

[Term]
id: INV:0000000
name: INVENTORY ROOT
namespace: INV

[Term] 
id: INV:0000001
name: Abiotic Stress
def: "Abiotic Stress" []
namespace: INV
is_a: INV:0000000 ! ROOT

[Term] 
id: INV:0000002
name: Agronomic
def: "Agronomic" []
namespace: INV
is_a: INV:0000000 ! ROOT

[Term] 
id: INV:0000003
name: Biotic Stress
def: "Biotic Stress" []
namespace: INV
is_a: INV:0000000 ! ROOT

[Term] 
id: INV:0000004
name: Morphological
def: "Morphological" []
namespace: INV
is_a: INV:0000000 ! ROOT

[Term] 
id: INV:0000005
name: Physiological
def: "Physiological" []
namespace: INV
is_a: INV:0000000 ! ROOT

[Term] 
id: INV:0000006
name: Quality
def: "Quality" []
namespace: INV
is_a: INV:0000000 ! ROOT

[Term] 
id: INV:0000007
name: Acid
def: "" []
namespace: INV
is_a: INV:0000006 ! Quality

[Term] 
id: INV:0000008
name: Biological Index Inoculation Date
def: "" []
namespace: INV
is_a: INV:0000003 ! Biotic Stress

[Term] 
id: INV:0000009
name: Biological Index Inoculation Source Tree
def: "" []
namespace: INV
is_a: INV:0000003 ! Biotic Stress

[Term] 
id: INV:0000010
name: Biological Index Result
def: "" []
namespace: INV
is_a: INV:0000003 ! Biotic Stress

[Term] 
id: INV:0000011
name: Brix Acid Ratio
def: "" []
namespace: INV
is_a: INV:0000006 ! Quality

[Term] 
id: INV:0000012
name: Canopy Color
def: "" []
namespace: INV
is_a: INV:0000004 ! Morphological

[Term] 
id: INV:0000013
name: Canopy Density
def: "" []
namespace: INV
is_a: INV:0000004 ! Morphological

[Term] 
id: INV:0000014
name: Canopy Diameter
def: "" []
namespace: INV
is_a: INV:0000004 ! Morphological

[Term] 
id: INV:0000015
name: Canopy Volume
def: "" []
namespace: INV
is_a: INV:0000004 ! Morphological

[Term] 
id: INV:0000016
name: Chopped Fruit Weight
def: "" []
namespace: INV
is_a: INV:0000004 ! Morphological

[Term] 
id: INV:0000017
name: Days to Recover
def: "" []
namespace: INV
is_a: INV:0000001 ! Abiotic Stress

[Term] 
id: INV:0000018
name: Days to Wilt
def: "" []
namespace: INV
is_a: INV:0000001 ! Abiotic Stress

[Term] 
id: INV:0000019
name: Dry Fruit Weight
def: "" []
namespace: INV
is_a: INV:0000004 ! Morphological

[Term] 
id: INV:0000020
name: Dry Leaf Weight
def: "" []
namespace: INV
is_a: INV:0000004 ! Morphological

[Term] 
id: INV:0000021
name: Dry Seed Weight
def: "" []
namespace: INV
is_a: INV:0000004 ! Morphological

[Term] 
id: INV:0000022
name: Dry Soil Weight
def: "" []
namespace: INV
is_a: INV:0000001 ! Abiotic Stress

[Term] 
id: INV:0000023
name: Endocarp Color
def: "" []
namespace: INV
is_a: INV:0000004 ! Morphological

[Term] 
id: INV:0000024
name: Exocarp Color
def: "" []
namespace: INV
is_a: INV:0000004 ! Morphological

[Term] 
id: INV:0000025
name: Exocarp Texture
def: "" []
namespace: INV
is_a: INV:0000004 ! Morphological

[Term] 
id: INV:0000026
name: Exocarp Thickness
def: "" []
namespace: INV
is_a: INV:0000004 ! Morphological

[Term] 
id: INV:0000027
name: Final Fruit Temperature
def: "" []
namespace: INV
is_a: INV:0000005 ! Physiological

[Term] 
id: INV:0000028
name: Fresh Fruit Weight
def: "" []
namespace: INV
is_a: INV:0000004 ! Morphological

[Term] 
id: INV:0000029
name: Fresh Leaf Weight
def: "" []
namespace: INV
is_a: INV:0000004 ! Morphological

[Term] 
id: INV:0000030
name: Fresh Seed Weight
def: "" []
namespace: INV
is_a: INV:0000004 ! Morphological

[Term] 
id: INV:0000031
name: Fruit Area
def: "" []
namespace: INV
is_a: INV:0000004 ! Morphological

[Term] 
id: INV:0000032
name: Fruit Collection Date
def: "" []
namespace: INV
is_a: INV:0000004 ! Morphological

[Term] 
id: INV:0000033
name: Fruit Diameter
def: "" []
namespace: INV
is_a: INV:0000004 ! Morphological

[Term] 
id: INV:0000034
name: Fruit Longest Path
def: "" []
namespace: INV
is_a: INV:0000004 ! Morphological

[Term] 
id: INV:0000035
name: Fruit Perimeter
def: "" []
namespace: INV
is_a: INV:0000004 ! Morphological

[Term] 
id: INV:0000036
name: Fruit Volume
def: "" []
namespace: INV
is_a: INV:0000004 ! Morphological

[Term] 
id: INV:0000037
name: Fruit Water Activity
def: "" []
namespace: INV
is_a: INV:0000005 ! Physiological

[Term] 
id: INV:0000038
name: Fruit Water Loss
def: "" []
namespace: INV
is_a: INV:0000001 ! Abiotic Stress

[Term] 
id: INV:0000039
name: Fruit Water Potential
def: "" []
namespace: INV
is_a: INV:0000005 ! Physiological

[Term] 
id: INV:0000040
name: Graft Survival
def: "" []
namespace: INV
is_a: INV:0000002 ! Agronomic

[Term] 
id: INV:0000041
name: Graft Survival Date
def: "" []
namespace: INV
is_a: INV:0000002 ! Agronomic

[Term] 
id: INV:0000042
name: Juice Percent
def: "" []
namespace: INV
is_a: INV:0000006 ! Quality

[Term] 
id: INV:0000043
name: Juice Weight
def: "" []
namespace: INV
is_a: INV:0000002 ! Agronomic

[Term] 
id: INV:0000044
name: Leaf Collection Date
def: "" []
namespace: INV
is_a: INV:0000004 ! Morphological

[Term] 
id: INV:0000045
name: Leaf Conductance
def: "" []
namespace: INV
is_a: INV:0000005 ! Physiological

[Term] 
id: INV:0000046
name: Leaf Relative Humidity
def: "" []
namespace: INV
is_a: INV:0000005 ! Physiological

[Term] 
id: INV:0000047
name: Leaf Relative Water Content
def: "" []
namespace: INV
is_a: INV:0000005 ! Physiological

[Term] 
id: INV:0000048
name: Leaf Water Loss
def: "" []
namespace: INV
is_a: INV:0000001 ! Abiotic Stress

[Term] 
id: INV:0000049
name: Rootstock Trunk Diameter
def: "" []
namespace: INV
is_a: INV:0000004 ! Morphological

[Term] 
id: INV:0000050
name: Sampled Fruit Number
def: "" []
namespace: INV
is_a: INV:0000002 ! Agronomic

[Term] 
id: INV:0000051
name: Scion Trunk Diameter
def: "" []
namespace: INV
is_a: INV:0000004 ! Morphological

[Term] 
id: INV:0000052
name: Seed Count
def: "" []
namespace: INV
is_a: INV:0000006 ! Quality

[Term] 
id: INV:0000053
name: Seed Water Loss
def: "" []
namespace: INV
is_a: INV:0000001 ! Abiotic Stress

[Term] 
id: INV:0000054
name: Soil Moisture
def: "" []
namespace: INV
is_a: INV:0000001 ! Abiotic Stress

[Term] 
id: INV:0000055
name: Total Soluble Solids
def: "" []
namespace: INV
is_a: INV:0000006 ! Quality

[Term] 
id: INV:0000056
name: Tree Yield
def: "" []
namespace: INV
is_a: INV:0000002 ! Agronomic

[Term] 
id: INV:0000057
name: Turgid Leaf Weight
def: "" []
namespace: INV
is_a: INV:0000004 ! Morphological

[Term] 
id: INV:0000058
name: Wet Soil Weight
def: "" []
namespace: INV
is_a: INV:0000001 ! Abiotic Stress


###The trait for ID: INV:0000059 (Name:Acid - Measurement - pH), could you please change the definition to: "Juice acidity from fruit sample using a pH meter" and change the synonym to only Acid_pH.

[Term] 
id: INV:0000059
name: Acid - Measurement - pH
def: "Juice acidity from fruit sample using a pH meter" []
synonym: "Acid_pH" EXACT []
namespace: INV
relationship: variable_of INV:0000007 ! Acid

[Term] 
id: INV:0000060
name: Biological Index Inoculation - Date - YYYY-MM-DD
def: "Date tree was inoculated with pathogen for bioindexing - YYYY-MM-DD" []
synonym: "BioIdxDate_ymd" EXACT []
namespace: INV
relationship: variable_of INV:0000008 ! Biological Index Inoculation Date

[Term] 
id: INV:0000061
name: Biological Index Inoculation Source Tree - Text
def: "Unique identifier of positive source tree used for inoculation." []
synonym: "BioIdxSrcTree_txt" EXACT []
namespace: INV
relationship: variable_of INV:0000009 ! Biological Index Inoculation Source Tree

[Term] 
id: INV:0000062
name: Biological Index Result - Rating
def: "Visual rating of bioindexing result" []
synonym: "BioIdxRes_Rate_brs" EXACT []
namespace: INV
relationship: variable_of INV:0000010 ! Biological Index Result

[Term] 
id: INV:0000063
name: Brix Acid Ratio - Calculation
def: "Brix/TSS measurement divided by Titratable Acidity Measurement" []
synonym: "TSSAcidRat_Comp" EXACT []
namespace: INV
relationship: variable_of INV:0000011 ! Brix Acid Ratio

[Term] 
id: INV:0000064
name: Canopy Color - Rating - 1-5 Color Scale
def: "Rating of overall color of canopy from 1 to 5, where 1=very yellow, worst and 5=very green, best." []
synonym: "CnpyCol_Rate_1to5" EXACT []
namespace: INV
relationship: variable_of INV:0000012 ! Canopy Color

[Term] 
id: INV:0000065
name: Canopy Density - Digital Canopy Analyzer Measurement - LAI
def: "Tree Canopy Density Measurement using Digital Canopy Analyzer (LAI)" []
synonym: "CnpyDns_LAI" EXACT []
namespace: INV
relationship: variable_of INV:0000013 ! Canopy Density

[Term] 
id: INV:0000066
name: Canopy Diameter - East to West - centimeters
def: "Canopy width measurement from East to West in cm." []
synonym: "CnpyDia_EW_cm" EXACT []
namespace: INV
relationship: variable_of INV:0000014 ! Canopy Diameter

[Term] 
id: INV:0000067
name: Canopy Diameter - North to South - centimeters
def: "Canopy width measurement from North to South in cm." []
synonym: "CnpyDia_NS_cm" EXACT []
namespace: INV
relationship: variable_of INV:0000014 ! Canopy Diameter

[Term] 
id: INV:0000068
name: Canopy Volume - Calculation - m^3
def: "Calculation of canopy volume based on Canopy Diameter from N-S, Canopy Diameter from E-W, and Height of Tree in m3. (NS_Dia*EW_Dia*TreeHt)/4" []
synonym: "CnpyVol_Comp_m3" EXACT []
namespace: INV
relationship: variable_of INV:0000015 ! Canopy Volume

[Term] 
id: INV:0000069
name: Chopped Fruit Weight - Measurement - grams
def: "Fruit sample weight after chopping for evaluation  in grams." []
synonym: "ChpFrtWt_g" EXACT []
namespace: INV
relationship: variable_of INV:0000016 ! Chopped Fruit Weight

[Term] 
id: INV:0000070
name: Days to Recover - count
def: "A count of the number of days after water reintroduction until tree recovers." []
synonym: "Days2Rcvr_Cnt" EXACT []
namespace: INV
relationship: variable_of INV:0000017 ! Days to Recover

[Term] 
id: INV:0000071
name: Days to Wilt - count
def: "A count of the number of days after drought conditions are applied until tree wilts." []
synonym: "Days2Wilt_Cnt" EXACT []
namespace: INV
relationship: variable_of INV:0000018 ! Days to Wilt

[Term] 
id: INV:0000072
name: Dry Fruit Weight - Measurement - grams
def: "Fruit sample weight after drying in grams." []
synonym: "DryFrtWt_g" EXACT []
namespace: INV
relationship: variable_of INV:0000019 ! Dry Fruit Weight

[Term] 
id: INV:0000073
name: Dry Leaf Weight - Measurement - grams
def: "Leaf sample weight in grams after drying in oven at 85C overnight" []
synonym: "DryLfWt_g" EXACT []
namespace: INV
relationship: variable_of INV:0000020 ! Dry Leaf Weight

[Term] 
id: INV:0000074
name: Dry Seed Weight - Measurement - grams
def: "Seed sample weight in grams after drying." []
synonym: "DrySdWt_g" EXACT []
namespace: INV
relationship: variable_of INV:0000021 ! Dry Seed Weight

[Term] 
id: INV:0000075
name: Dry Soil Weight - Measurement - grams
def: "Direct measurement of the weight in grams of a soil sample after drying." []
synonym: "DrySoilWt_g" EXACT []
namespace: INV
relationship: variable_of INV:0000022 ! Dry Soil Weight

[Term] 
id: INV:0000076
name: Endocarp Color - Class 1 Color Percentage
def: "Percentage of pixels assigned to class 1 color bin (RGB 173 90 32) using Naïve Bayes. (# Assigned Pixels)/(Total # Pixels)" []
synonym: "EndoCol_Cls1_pct" EXACT []
namespace: INV
relationship: variable_of INV:0000023 ! Endocarp Color

[Term] 
id: INV:0000077
name: Endocarp Color - Class 1 Color Pixel Count
def: "Number of pixels assigned to class 1 color bin (RGB 173 90 32) using Naïve Bayes." []
synonym: "EndoCol_Cls1Px_ct" EXACT []
namespace: INV
relationship: variable_of INV:0000023 ! Endocarp Color

[Term] 
id: INV:0000078
name: Endocarp Color - Class 10 Color Percentage
def: "Percentage of pixels assigned to class 10 color bin (RGB 173 90 32) using Naïve Bayes. (# Assigned Pixels)/(Total # Pixels)" []
synonym: "EndoCol_Cls10_pct" EXACT []
namespace: INV
relationship: variable_of INV:0000023 ! Endocarp Color

[Term] 
id: INV:0000079
name: Endocarp Color - Class 10 Color Pixel Count
def: "Number of pixels assigned to class 10 color bin (RGB 173 90 32) using Naïve Bayes." []
synonym: "EndoCol_Cls10Px_ct" EXACT []
namespace: INV
relationship: variable_of INV:0000023 ! Endocarp Color

[Term] 
id: INV:0000080
name: Endocarp Color - Class 2 Color Percentage
def: "Percentage of pixels assigned to class 2 color bin (RGB 173 90 32) using Naïve Bayes. (# Assigned Pixels)/(Total # Pixels)" []
synonym: "EndoCol_Cls2_pct" EXACT []
namespace: INV
relationship: variable_of INV:0000023 ! Endocarp Color

[Term] 
id: INV:0000081
name: Endocarp Color - Class 2 Color Pixel Count
def: "Number of pixels assigned to class 2 color bin (RGB 173 90 32) using Naïve Bayes." []
synonym: "EndoCol_Cls2Px_ct" EXACT []
namespace: INV
relationship: variable_of INV:0000023 ! Endocarp Color

[Term] 
id: INV:0000082
name: Endocarp Color - Class 3 Color Percentage
def: "Percentage of pixels assigned to class 3 color bin (RGB 173 90 32) using Naïve Bayes. (# Assigned Pixels)/(Total # Pixels)" []
synonym: "EndoCol_Cls3_pct" EXACT []
namespace: INV
relationship: variable_of INV:0000023 ! Endocarp Color

[Term] 
id: INV:0000083
name: Endocarp Color - Class 3 Color Pixel Count
def: "Number of pixels assigned to class 3 color bin (RGB 173 90 32) using Naïve Bayes." []
synonym: "EndoCol_Cls3Px_ct" EXACT []
namespace: INV
relationship: variable_of INV:0000023 ! Endocarp Color

[Term] 
id: INV:0000084
name: Endocarp Color - Class 6 Color Percentage
def: "Percentage of pixels assigned to class 6 color bin (RGB 173 90 32) using Naïve Bayes. (# Assigned Pixels)/(Total # Pixels)" []
synonym: "EndoCol_Cls6_pct" EXACT []
namespace: INV
relationship: variable_of INV:0000023 ! Endocarp Color

[Term] 
id: INV:0000085
name: Endocarp Color - Class 6 Color Pixel Count
def: "Number of pixels assigned to class 6 color bin (RGB 173 90 32) using Naïve Bayes." []
synonym: "EndoCol_Cls6Px_ct" EXACT []
namespace: INV
relationship: variable_of INV:0000023 ! Endocarp Color

[Term] 
id: INV:0000086
name: Endocarp Color - Class 8 Color Percentage
def: "Percentage of pixels assigned to class 8 color bin (RGB 173 90 32) using Naïve Bayes. (# Assigned Pixels)/(Total # Pixels)" []
synonym: "EndoCol_Cls8_pct" EXACT []
namespace: INV
relationship: variable_of INV:0000023 ! Endocarp Color

[Term] 
id: INV:0000087
name: Endocarp Color - Class 8 Color Pixel Count
def: "Number of pixels assigned to class 8 color bin (RGB 173 90 32) using Naïve Bayes." []
synonym: "EndoCol_Cls8Px_ct" EXACT []
namespace: INV
relationship: variable_of INV:0000023 ! Endocarp Color

[Term] 
id: INV:0000088
name: Endocarp Color - Rating - 0-7 Endocarp Fruit Color Scale
def: "Estimation of endocarp color using a rating scale" []
synonym: "EndCol_Rate_endo" EXACT []
namespace: INV
relationship: variable_of INV:0000023 ! Endocarp Color

[Term] 
id: INV:0000089
name: Exocarp Color - Class 1 Color Percentage
def: "Percentage of pixels assigned to class 1 color bin (RGB 173 90 32) using Naïve Bayes. (# Assigned Pixels)/(Total # Pixels)" []
synonym: "ExoCol_Cls1_pct" EXACT []
namespace: INV
relationship: variable_of INV:0000024 ! Exocarp Color

[Term] 
id: INV:0000090
name: Exocarp Color - Class 1 Color Pixel Count
def: "Number of pixels assigned to class 1 color bin (RGB 173 90 32) using Naïve Bayes." []
synonym: "ExoCol_Cls1Px_ct" EXACT []
namespace: INV
relationship: variable_of INV:0000024 ! Exocarp Color

[Term] 
id: INV:0000091
name: Exocarp Color - Class 10 Color Percentage
def: "Percentage of pixels assigned to class 10 color bin (RGB 173 90 32) using Naïve Bayes. (# Assigned Pixels)/(Total # Pixels)" []
synonym: "ExoCol_Cls10_pct" EXACT []
namespace: INV
relationship: variable_of INV:0000024 ! Exocarp Color

[Term] 
id: INV:0000092
name: Exocarp Color - Class 10 Color Pixel Count
def: "Number of pixels assigned to class 10 color bin (RGB 173 90 32) using Naïve Bayes." []
synonym: "ExoCol_Cls10Px_ct" EXACT []
namespace: INV
relationship: variable_of INV:0000024 ! Exocarp Color

[Term] 
id: INV:0000093
name: Exocarp Color - Class 2 Color Percentage
def: "Percentage of pixels assigned to class 2 color bin (RGB 173 90 32) using Naïve Bayes. (# Assigned Pixels)/(Total # Pixels)" []
synonym: "ExoCol_Cls2_pct" EXACT []
namespace: INV
relationship: variable_of INV:0000024 ! Exocarp Color

[Term] 
id: INV:0000094
name: Exocarp Color - Class 2 Color Pixel Count
def: "Number of pixels assigned to class 2 color bin (RGB 173 90 32) using Naïve Bayes." []
synonym: "ExoCol_Cls2Px_ct" EXACT []
namespace: INV
relationship: variable_of INV:0000024 ! Exocarp Color

[Term] 
id: INV:0000095
name: Exocarp Color - Class 3 Color Percentage
def: "Percentage of pixels assigned to class 3 color bin (RGB 173 90 32) using Naïve Bayes. (# Assigned Pixels)/(Total # Pixels)" []
synonym: "ExoCol_Cls3_pct" EXACT []
namespace: INV
relationship: variable_of INV:0000024 ! Exocarp Color

[Term] 
id: INV:0000096
name: Exocarp Color - Class 3 Color Pixel Count
def: "Number of pixels assigned to class 3 color bin (RGB 173 90 32) using Naïve Bayes." []
synonym: "ExoCol_Cls3Px_ct" EXACT []
namespace: INV
relationship: variable_of INV:0000024 ! Exocarp Color

[Term] 
id: INV:0000097
name: Exocarp Color - Class 6 Color Percentage
def: "Percentage of pixels assigned to class 6 color bin (RGB 173 90 32) using Naïve Bayes. (# Assigned Pixels)/(Total # Pixels)" []
synonym: "ExoCol_Cls6_pct" EXACT []
namespace: INV
relationship: variable_of INV:0000024 ! Exocarp Color

[Term] 
id: INV:0000098
name: Exocarp Color - Class 6 Color Pixel Count
def: "Number of pixels assigned to class 6 color bin (RGB 173 90 32) using Naïve Bayes." []
synonym: "ExoCol_Cls6Px_ct" EXACT []
namespace: INV
relationship: variable_of INV:0000024 ! Exocarp Color

[Term] 
id: INV:0000099
name: Exocarp Color - Class 8 Color Percentage
def: "Percentage of pixels assigned to class 8 color bin (RGB 173 90 32) using Naïve Bayes. (# Assigned Pixels)/(Total # Pixels)" []
synonym: "ExoCol_Cls8_pct" EXACT []
namespace: INV
relationship: variable_of INV:0000024 ! Exocarp Color

[Term] 
id: INV:0000100
name: Exocarp Color - Class 8 Color Pixel Count
def: "Number of pixels assigned to class 8 color bin (RGB 173 90 32) using Naïve Bayes." []
synonym: "ExoCol_Cls8Px_ct" EXACT []
namespace: INV
relationship: variable_of INV:0000024 ! Exocarp Color

[Term] 
id: INV:0000101
name: Exocarp Color - Rating - 3-13 Exocarp Fruit Color Scale
def: "Rating of exocarp color based on color reference chart from 3 to 13, where 3 = Dark Green, 5 = Color Break, and 13 = Orange Red." []
synonym: "ExoCol_Rate_3to13" EXACT []
namespace: INV
relationship: variable_of INV:0000024 ! Exocarp Color

[Term] 
id: INV:0000102
name: Exocarp Texture - Rating - 1-8 Exocarp Texture Scale
def: "Exocarp texture estimation of fruit sample using a rating scale from 1 to 8, where 1 = Smooth and 8 = Rough." []
synonym: "ExoTxt_Rate_1to8" EXACT []
namespace: INV
relationship: variable_of INV:0000025 ! Exocarp Texture

[Term] 
id: INV:0000103
name: Exocarp Thickness - Single Fruit - millimeters
def: "Exocarp (rind) thickness in mm of a single fruit." []
synonym: "ExoSingleThck_mm" EXACT []
namespace: INV
relationship: variable_of INV:0000026 ! Exocarp Thickness

[Term] 
id: INV:0000104
name: Exocarp Thickness - Total Sample - millimeters
def: "Total exocarp (rind) thickness in mm of a group of fruit in fruit sample." []
synonym: "ExoTotThck_mm" EXACT []
namespace: INV
relationship: variable_of INV:0000026 ! Exocarp Thickness

[Term] 
id: INV:0000105
name: Final Fruit Temperature - Aqualab 4TE - Degrees Celsius
def: "Final fruit temperature in degrees Celsius using the Aqualab 4TE meter." []
synonym: "FrtTempFin_Aqua_degC" EXACT []
namespace: INV
relationship: variable_of INV:0000027 ! Final Fruit Temperature

[Term] 
id: INV:0000106
name: Final Fruit Temperature - WP4C - Degrees Celsius
def: "Final fruit temperature in degrees Celsius using the WP4C Dewpoint PotentiaMeter." []
synonym: "FrtTempFin_WP4C_degC" EXACT []
namespace: INV
relationship: variable_of INV:0000027 ! Final Fruit Temperature

[Term] 
id: INV:0000107
name: Fresh Fruit Weight - Measurement - grams
def: "Weight of all fruit in sample in grams." []
synonym: "FrshFrtWt_g" EXACT []
namespace: INV
relationship: variable_of INV:0000028 ! Fresh Fruit Weight

[Term] 
id: INV:0000108
name: Fresh Fruit Weight - Measurement - kilograms
def: "Weight of all fruit in sample in kilograms." []
synonym: "FrshFrtWt_kg" EXACT []
namespace: INV
relationship: variable_of INV:0000028 ! Fresh Fruit Weight

[Term] 
id: INV:0000109
name: Fresh Leaf Weight - Measurement - grams
def: "Fresh leaf sample weight in grams." []
synonym: "FrshLfWt_g" EXACT []
namespace: INV
relationship: variable_of INV:0000029 ! Fresh Leaf Weight

[Term] 
id: INV:0000110
name: Fresh Seed Weight - Measurement - grams
def: "Fresh seed sample weight in grams." []
synonym: "FrshSdWt_g" EXACT []
namespace: INV
relationship: variable_of INV:0000030 ! Fresh Seed Weight

[Term] 
id: INV:0000111
name: Fruit Area - Area of Convex Hull of Fruit from Cut Side Down Image - mm^2
def: "Fruit is cut in half and imaged cut side down. A convex hull is fitted on fruit and area is measured in mm2" []
synonym: "FrtArea_CutDnCvxHul_mm2" EXACT []
namespace: INV
relationship: variable_of INV:0000031 ! Fruit Area

[Term] 
id: INV:0000112
name: Fruit Area - Area of Convex Hull of Fruit from Cut Side Up Image - mm^2
def: "Fruit is cut in half and imaged cut side up. A convex hull is fitted on fruit and area is measured in mm2" []
synonym: "FrtArea_CutUpCvxHul_mm2" EXACT []
namespace: INV
relationship: variable_of INV:0000031 ! Fruit Area

[Term] 
id: INV:0000113
name: Fruit Area - From Cut Side Down Image - mm^2
def: "Fruit is cut in half and imaged cut side down and area of entire surface is measured in mm2" []
synonym: "FrtArea_CutDn_mm2" EXACT []
namespace: INV
relationship: variable_of INV:0000031 ! Fruit Area

[Term] 
id: INV:0000114
name: Fruit Area - From Cut Side Up Image - mm^2
def: "Fruit is cut in half and imaged cut side up and area of entire surface is measured in mm2" []
synonym: "FrtArea_CutUp_mm2" EXACT []
namespace: INV
relationship: variable_of INV:0000031 ! Fruit Area

[Term] 
id: INV:0000115
name: Fruit Collection Date - YYYY-MM-DD
def: "Date fruit sample was collected." []
synonym: "FrtClctDate_Mst_ymd" EXACT []
namespace: INV
relationship: variable_of INV:0000032 ! Fruit Collection Date

[Term] 
id: INV:0000116
name: Fruit Diameter - Ellipse Major Axis from Cut Side Down Fruit Image - millimeters
def: "Fruit is cut in half and imaged cut side down. An ellipse is fitted to fruit and the length of the major axis of ellipse is measured in mm." []
synonym: "FrtDia_CutDnElpsMaj_mm" EXACT []
namespace: INV
relationship: variable_of INV:0000033 ! Fruit Diameter

[Term] 
id: INV:0000117
name: Fruit Diameter - Ellipse Major Axis from Cut Side Up Fruit Image- millimeters
def: "Fruit is cut in half and imaged cut side up. An ellipse is fitted to fruit and the length of the major axis of ellipse is measured in mm" []
synonym: "FrtDia_CutUpElpsMaj_mm" EXACT []
namespace: INV
relationship: variable_of INV:0000033 ! Fruit Diameter

[Term] 
id: INV:0000118
name: Fruit Diameter - Ellipse Major Axis from Side 1 of Whole Fruit Imaged with Poles Parallel - millimeters
def: "Whole fruit is imaged on a single side (side 1) with poles oriented parallel to background surface. An ellipse is fitted to fruit and the length of the major axis of ellipse is measured in mm" []
synonym: "FrtDia_WVElpsMajS1_mm" EXACT []
namespace: INV
relationship: variable_of INV:0000033 ! Fruit Diameter

[Term] 
id: INV:0000119
name: Fruit Diameter - Ellipse Major Axis from Side 1 of Whole Fruit Imaged with Poles Perpendicular - millimeters
def: "Whole fruit is imaged on a single side (side 1) with poles oriented perpendicular to background surface. An ellipse is fitted to fruit and the length of the major axis of ellipse is measured in mm" []
synonym: "FrtDia_WHElpsMajS1_mm" EXACT []
namespace: INV
relationship: variable_of INV:0000033 ! Fruit Diameter

[Term] 
id: INV:0000120
name: Fruit Diameter - Ellipse Major Axis from Side 2 of Whole Fruit Imaged with Poles Parallel - millimeters
def: "Whole fruit is imaged on side 2 (180 degree rotation from side 1) with poles oriented parallel to background surface. An ellipse is fitted to fruit and the length of the major axis of ellipse is measured in mm" []
synonym: "FrtDia_WVElpsMajS2_mm" EXACT []
namespace: INV
relationship: variable_of INV:0000033 ! Fruit Diameter

[Term] 
id: INV:0000121
name: Fruit Diameter - Ellipse Major Axis from Side 2 of Whole Fruit Imaged with Poles Perpendicular - millimeters
def: "Whole fruit is imaged on side 2 (180 degree rotation from side 1) with poles oriented perpendicular to background surface. An ellipse is fitted to fruit and the length of the major axis of ellipse is measured in mm" []
synonym: "FrtDia_WHElpsMajS2_mm" EXACT []
namespace: INV
relationship: variable_of INV:0000033 ! Fruit Diameter

[Term] 
id: INV:0000122
name: Fruit Diameter - Ellipse Minor Axis from Cut Side Down Fruit Image - millimeters
def: "Fruit is cut in half and imaged cut side down. An ellipse is fitted to fruit and the length of the minor axis of ellipse is measured in mm" []
synonym: "FrtDia_CutDnElpsMin_mm" EXACT []
namespace: INV
relationship: variable_of INV:0000033 ! Fruit Diameter

[Term] 
id: INV:0000123
name: Fruit Diameter - Ellipse Minor Axis from Cut Side Up Fruit Image - millimeters
def: "Fruit is cut in half and imaged cut side up. An ellipse is fitted to fruit and the length of the minor axis of ellipse is measured in mm" []
synonym: "FrtDia_CutUpElpsMin_mm" EXACT []
namespace: INV
relationship: variable_of INV:0000033 ! Fruit Diameter

[Term] 
id: INV:0000124
name: Fruit Diameter - Ellipse Minor Axis from Side 1 of Whole Fruit Imaged with Poles Parallel - millimeters
def: "Whole fruit is imaged on a single side (side 1) with oriented parallel to background surface. An ellipse is fitted to fruit and the length of the minor axis of ellipse is measured in mm" []
synonym: "FrtDia_WVElpsMinS1_mm" EXACT []
namespace: INV
relationship: variable_of INV:0000033 ! Fruit Diameter

[Term] 
id: INV:0000125
name: Fruit Diameter - Ellipse Minor Axis from Side 1 of Whole Fruit Imaged with Poles Perpendicular - millimeters
def: "Whole fruit is imaged on a single side (side 1) with poles oriented perpendicular to background surface. An ellipse is fitted to fruit and the length of the minor axis of ellipse is measured in mm" []
synonym: "FrtDia_WHElpsMinS1_mm" EXACT []
namespace: INV
relationship: variable_of INV:0000033 ! Fruit Diameter

[Term] 
id: INV:0000126
name: Fruit Diameter - Ellipse Minor Axis from Side 2 of Whole Fruit Imaged with Poles Parallel - millimeters
def: "Whole fruit is imaged on side 2 (180 degree rotation from side 1) with poles oriented parallel to background surface. An ellipse is fitted to fruit and the length of the minor axis of ellipse is measured in mm" []
synonym: "FrtDia_WVElpsMinS2_mm" EXACT []
namespace: INV
relationship: variable_of INV:0000033 ! Fruit Diameter

[Term] 
id: INV:0000127
name: Fruit Diameter - Ellipse Minor Axis from Side 2 of Whole Fruit Imaged with Poles Perpendicular - millimeters
def: "Whole fruit is imaged on side 2 (180 degree rotation from side 1) with poles oriented perpendicular to background surface. An ellipse is fitted to fruit and the length of the minor axis of ellipse is measured in mm" []
synonym: "FrtDia_WHElpsMinS2_mm" EXACT []
namespace: INV
relationship: variable_of INV:0000033 ! Fruit Diameter

[Term] 
id: INV:0000128
name: Fruit Diameter - Height from Cut Side Down Fruit Image - millimeters
def: "Fruit is cut in half and imaged cut side down. The verticle axis (height) is measured from furthest point on top and furthest point on bottom of fruit in mm" []
synonym: "FrtDia_CutDnHeight_mm" EXACT []
namespace: INV
relationship: variable_of INV:0000033 ! Fruit Diameter

[Term] 
id: INV:0000129
name: Fruit Diameter - Height from Cut Side Up Fruit Image - millimeters
def: "Fruit is cut in half and imaged cut side up. The verticle axis (height) is measured from furthest point on top and furthest point on bottom of fruit in mm" []
synonym: "FrtDia_CutUpHeight_mm" EXACT []
namespace: INV
relationship: variable_of INV:0000033 ! Fruit Diameter

[Term] 
id: INV:0000130
name: Fruit Diameter - Height from Side 1 of Whole Fruit Imaged with Poles Parallel - millimeters
def: "Whole fruit is imaged on a single side (side 1) with poles oriented parallel to background surface. The verticle axis (height) is measured from furthest point on top and furthest point on bottom of fruit in mm" []
synonym: "FrtDia_WVHeightS1_mm" EXACT []
namespace: INV
relationship: variable_of INV:0000033 ! Fruit Diameter

[Term] 
id: INV:0000131
name: Fruit Diameter - Height from Side 1 of Whole Fruit Imaged with Poles Perpendicular - millimeters
def: "Whole fruit is imaged on a single side (side 1) with poles oriented perpendicular to background surface. The verticle axis (height) is measured from furthest point on top and furthest point on bottom of fruit in mm" []
synonym: "FrtDia_WHHeightS1_mm" EXACT []
namespace: INV
relationship: variable_of INV:0000033 ! Fruit Diameter

[Term] 
id: INV:0000132
name: Fruit Diameter - Height from Side 2 of Whole Fruit Imaged with Poles Parallel - millimeters
def: "Whole fruit is imaged on side 2 (180 degree rotation from side 1) with poles oriented parallel to background surface. The verticle axis (height) is measured from furthest point on top and furthest point on bottom of fruit in mm" []
synonym: "FrtDia_WVHeightS2_mm" EXACT []
namespace: INV
relationship: variable_of INV:0000033 ! Fruit Diameter

[Term] 
id: INV:0000133
name: Fruit Diameter - Height from Side 2 of Whole Fruit Imaged with Poles Perpendicular - millimeters
def: "Whole fruit is imaged on side 2 (180 degree rotation from side 1) with poles oriented perpendicular to background surface. The verticle axis (height) is measured from furthest point on top and furthest point on bottom of fruit in mm" []
synonym: "FrtDia_WHHeightS2_mm" EXACT []
namespace: INV
relationship: variable_of INV:0000033 ! Fruit Diameter

[Term] 
id: INV:0000134
name: Fruit Diameter - Manual Equatorial - centimeters
def: "Equatorial diameter of fruit sample manually measured in cm." []
synonym: "FrtDia_EquMan_cm" EXACT []
namespace: INV
relationship: variable_of INV:0000033 ! Fruit Diameter

[Term] 
id: INV:0000135
name: Fruit Diameter - Manual Equatorial - millimeters
def: "Equatorial diameter of fruit sample manually measured in mm." []
synonym: "FrtDia_EquMan_mm" EXACT []
namespace: INV
relationship: variable_of INV:0000033 ! Fruit Diameter

[Term] 
id: INV:0000136
name: Fruit Diameter - Manual Measurement of Total Length of All Fruit Sampled - centimeters
def: "Measurement of the total length of all fruit in cm (polar diameter) in sample when lined up top-to-bottom" []
synonym: "FrtDia_TotalLength_cm" EXACT []
namespace: INV
relationship: variable_of INV:0000033 ! Fruit Diameter

[Term] 
id: INV:0000137
name: Fruit Diameter - Manual Measurement of Total Width of All Fruit Sampled - centimeters
def: "Measurement of the total width in cm of all fruit (equatorial diameter) in sample when lined up side-by-side." []
synonym: "FrtDia_TotalWidth_cm" EXACT []
namespace: INV
relationship: variable_of INV:0000033 ! Fruit Diameter

[Term] 
id: INV:0000138
name: Fruit Diameter - Manual Polar - centimeters
def: "Polar diameter of single fruit manually measured in cm." []
synonym: "FrtDia_PolMan_cm" EXACT []
namespace: INV
relationship: variable_of INV:0000033 ! Fruit Diameter

[Term] 
id: INV:0000139
name: Fruit Diameter - Manual Polar - millimeters
def: "Polar diameter of single fruit manually measured in mm." []
synonym: "FrtDia_PolMan_mm" EXACT []
namespace: INV
relationship: variable_of INV:0000033 ! Fruit Diameter

[Term] 
id: INV:0000140
name: Fruit Diameter - Width from Cut Side Down Fruit Image - millimeters
def: "Fruit is cut in half and imaged cut side down. The horizontal axis (width) is measured from furthest point on left and furthest point on right of fruit in mm" []
synonym: "FrtDia_CutDnWidth_mm" EXACT []
namespace: INV
relationship: variable_of INV:0000033 ! Fruit Diameter

[Term] 
id: INV:0000141
name: Fruit Diameter - Width from Cut Side Up Fruit Image - millimeters
def: "Fruit is cut in half and imaged cut side up. The horizontal axis (width) is measured from furthest point on left and furthest point on right of fruit in mm" []
synonym: "FrtDia_CutUpWidth_mm" EXACT []
namespace: INV
relationship: variable_of INV:0000033 ! Fruit Diameter

[Term] 
id: INV:0000142
name: Fruit Diameter - Width from Side 1 of Whole Fruit Imaged with Poles Parallel - millimeters
def: "Whole fruit is imaged on a single side (side 1) with poles oriented parallel to background surface. The horizontal axis (width) is measured from furthest point on left and furthest point on right of fruit in mm" []
synonym: "FrtDia_WVWidthS1_mm" EXACT []
namespace: INV
relationship: variable_of INV:0000033 ! Fruit Diameter

[Term] 
id: INV:0000143
name: Fruit Diameter - Width from Side 1 of Whole Fruit Imaged with Poles Perpendicular - millimeters
def: "Whole fruit is imaged on a single side (side 1) with poles oriented perpendicular to background surface. The horizontal axis (width) is measured from furthest point on left and furthest point on right of fruit in mm" []
synonym: "FrtDia_WHWidthS1_mm" EXACT []
namespace: INV
relationship: variable_of INV:0000033 ! Fruit Diameter

[Term] 
id: INV:0000144
name: Fruit Diameter - Width from Side 2 of Whole Fruit Imaged with Poles Parallel - millimeters
def: "Whole fruit is imaged on side 2 (180 degree rotation from side 1) with poles oriented parallel to background surface. The horizontal axis (width) is measured from furthest point on left and furthest point on right of fruit in mm" []
synonym: "FrtDia_WVWidthS2_mm" EXACT []
namespace: INV
relationship: variable_of INV:0000033 ! Fruit Diameter

[Term] 
id: INV:0000145
name: Fruit Diameter - Width from Side 2 of Whole Fruit Imaged with Poles Perpendicular - millimeters
def: "Whole fruit is imaged on side 2 (180 degree rotation from side 1) with poles oriented perpendicular to background surface. The horizontal axis (width) is measured from furthest point on left and furthest point on right of fruit in mm" []
synonym: "FrtDia_WHWidthS2_mm" EXACT []
namespace: INV
relationship: variable_of INV:0000033 ! Fruit Diameter

[Term] 
id: INV:0000146
name: Fruit Longest Path - The longest path through fruit imaged Cut Side Down - millimeters
def: "Fruit is cut in half and imaged cut side down and the length of the line through center of mass and furthest point on the convex hull around fruit is measured in mm" []
synonym: "FrtLPath_CutDn_mm" EXACT []
namespace: INV
relationship: variable_of INV:0000034 ! Fruit Longest Path

[Term] 
id: INV:0000147
name: Fruit Longest Path - The longest path through fruit imaged Cut Side Up - millimeters
def: "Fruit is cut in half and imaged cut side up and the length of the line through center of mass and furthest point on the convex hull around fruit is measured in mm" []
synonym: "FrtLPath_CutUp_mm" EXACT []
namespace: INV
relationship: variable_of INV:0000034 ! Fruit Longest Path

[Term] 
id: INV:0000148
name: Fruit Perimeter - Cut Side Down Image - millimeters
def: "Fruit is cut in half and imaged cut side down. The perimeter around outer edge of fruit is measured in mm" []
synonym: "FrtPrmtr_CutDn_mm" EXACT []
namespace: INV
relationship: variable_of INV:0000035 ! Fruit Perimeter

[Term] 
id: INV:0000149
name: Fruit Perimeter - Cut Side Up Image - millimeters
def: "Fruit is cut in half and imaged cut side up. The perimeter around outer edge of fruit is measured in mm" []
synonym: "FrtPrmtr_CutUp_mm" EXACT []
namespace: INV
relationship: variable_of INV:0000035 ! Fruit Perimeter

[Term] 
id: INV:0000150
name: Fruit Volume - Calculation of fruit using major axis of ellipse from Cut Side Up Image - mm^3
def: "Fruit is cut in half and imaged cut side down. Volume is calculated based on minor axis of the fitted ellipse in mm3 (V=(Ï€d^3)/6)" []
synonym: "FrtVol_CutDnMin_mm3" EXACT []
namespace: INV
relationship: variable_of INV:0000036 ! Fruit Volume

[Term] 
id: INV:0000151
name: Fruit Volume - Calculation using major axis of ellipse from Cut Side Down image - mm^3
def: "Fruit is cut in half and imaged cut side down. Volume is calculated based on major axis of the fitted ellipse in mm3 (V=(Ï€d^3)/6)" []
synonym: "FrtVol_CutDnMaj_mm3" EXACT []
namespace: INV
relationship: variable_of INV:0000036 ! Fruit Volume

[Term] 
id: INV:0000152
name: Fruit Volume - Calculation using major axis of ellipse from Cut Side Up Image - mm^3
def: "Fruit is cut in half and imaged cut side up. Volume is calculated based on major axis of the fitted ellipse in mm3 (V=(Ï€d^3)/6)" []
synonym: "FrtVol_CutUpMaj_mm3" EXACT []
namespace: INV
relationship: variable_of INV:0000036 ! Fruit Volume

[Term] 
id: INV:0000153
name: Fruit Volume - Calculation using minor axis of ellipse from Cut Side Up Image - mm^3
def: "Fruit is cut in half and imaged cut side up. Volume is calculated based on minor axis of the fitted ellipse in mm3 (V=(Ï€d^3)/6)" []
synonym: "FrtVol_CutUpMin_mm3" EXACT []
namespace: INV
relationship: variable_of INV:0000036 ! Fruit Volume

[Term] 
id: INV:0000154
name: Fruit Water Activity - Aqualab 4TE - Aw
def: "Fruit water activity using the Aqualab 4TE meter (Aw)." []
synonym: "FrtWatAct_Aqua_Aw" EXACT []
namespace: INV
relationship: variable_of INV:0000037 ! Fruit Water Activity

[Term] 
id: INV:0000155
name: Fruit Water Activity - WP4C - Aw
def: "Fruit water activity using the WP4C Dewpoint PotentiaMeter (Aw)." []
synonym: "FrtWatAct_Aw" EXACT []
namespace: INV
relationship: variable_of INV:0000037 ! Fruit Water Activity

[Term] 
id: INV:0000156
name: Fruit Water Loss - Calculation - Percentage
def: "Fruit water loss calculation as a percentage. WatLoss = (Fresh Weight - Dry Weight)/(Fresh Weight)" []
synonym: "FrtWatLoss_Comp_pct" EXACT []
namespace: INV
relationship: variable_of INV:0000038 ! Fruit Water Loss

[Term] 
id: INV:0000157
name: Fruit Water Potential - WP4C- Megapascal
def: "Fruit water potential using the WP4C Dewpoint PotentiaMeter in mPa." []
synonym: "FrtWatPot_WP4C_mPa" EXACT []
namespace: INV
relationship: variable_of INV:0000039 ! Fruit Water Potential

[Term] 
id: INV:0000158
name: Graft Survival Date - YYYY-MM-DD
def: "Date tree graft was evaluated for survival." []
synonym: "GrftSurvDate_ymd" EXACT []
namespace: INV
relationship: variable_of INV:0000041 ! Graft Survival Date

[Term] 
id: INV:0000159
name: Graft Survival Status - 0-1 Dead/Alive
def: "Survival status of tree graft." []
synonym: "GrftSurv_da" EXACT []
namespace: INV
relationship: variable_of INV:0000040 ! Graft Survival

[Term] 
id: INV:0000160
name: Juice Percent - Calculation - percentage
def: "Total Juice Weight divided by Total Fruit Weight for a Fruit Sample (percentage)." []
synonym: "JuicePct_Comp" EXACT []
namespace: INV
relationship: variable_of INV:0000042 ! Juice Percent

[Term] 
id: INV:0000161
name: Juice Weight - Whole Sample - grams
def: "Juice weight of a fruit sample in grams." []
synonym: "JucWt_g" EXACT []
namespace: INV
relationship: variable_of INV:0000043 ! Juice Weight

[Term] 
id: INV:0000162
name: Juice Weight - Whole Sample - kilograms
def: "Juice weight of a fruit sample in kilograms." []
synonym: "JuiceWt_kg" EXACT []
namespace: INV
relationship: variable_of INV:0000043 ! Juice Weight

[Term] 
id: INV:0000163
name: Leaf Collection Date - YYYY-MM-DD
def: "Date leaf sample was collected." []
synonym: "LfClctDate_ymd" EXACT []
namespace: INV
relationship: variable_of INV:0000044 ! Leaf Collection Date

[Term] 
id: INV:0000164
name: Leaf Conductance - mmol/(m²·s)
def: "Leaf conductance of sample using a leaf porometer in mmolm2s." []
synonym: "LeafG_mmolm2s" EXACT []
namespace: INV
relationship: variable_of INV:0000045 ! Leaf Conductance

[Term] 
id: INV:0000165
name: Leaf Relative Humidity - percentage
def: "Leaf relative humidity of sample using a leaf porometer as a percentage." []
synonym: "LfRelHum_pct" EXACT []
namespace: INV
relationship: variable_of INV:0000046 ! Leaf Relative Humidity

[Term] 
id: INV:0000166
name: Leaf Relative Water Content - Calculation - percentage
def: "Relative water content calculation of a leaf sample as a percentage. RWC = (fresh weight - dry weight)/(turgid weight - dry weight)" []
synonym: "LfRWC_Comp_pct" EXACT []
namespace: INV
relationship: variable_of INV:0000047 ! Leaf Relative Water Content

[Term] 
id: INV:0000167
name: Leaf Water Loss - Calculation - percentage
def: "Leaf water loss calculation as a percentage. WatLoss = (Fresh Weight - Dry Weight)/(Fresh Weight)" []
synonym: "LfWatLoss_Comp_pct" EXACT []
namespace: INV
relationship: variable_of INV:0000048 ! Leaf Water Loss

[Term] 
id: INV:0000168
name: Rootstock Trunk Diameter - East to West - centimeters
def: "Measurement of diameter just below bud union from East to West in cm." []
synonym: "RtStckDia_EW_cm" EXACT []
namespace: INV
relationship: variable_of INV:0000049 ! Rootstock Trunk Diameter

[Term] 
id: INV:0000169
name: Rootstock Trunk Diameter - East to West - inches
def: "Measurement of diameter just below bud union from East to West in inches." []
synonym: "RtStckDia_EW_in" EXACT []
namespace: INV
relationship: variable_of INV:0000049 ! Rootstock Trunk Diameter

[Term] 
id: INV:0000170
name: Rootstock Trunk Diameter - North to South - centimeters
def: "Measurement of diameter just below bud union from North to South in cm." []
synonym: "RtStckDia_NS_cm" EXACT []
namespace: INV
relationship: variable_of INV:0000049 ! Rootstock Trunk Diameter

[Term] 
id: INV:0000171
name: Rootstock Trunk Diameter - North to South - inches
def: "Measurement of diameter just below bud union from North to South in inches." []
synonym: "RtStckDia_NS_in" EXACT []
namespace: INV
relationship: variable_of INV:0000049 ! Rootstock Trunk Diameter

[Term] 
id: INV:0000172
name: Sampled Fruit Number - count
def: "The number of fruit in a sample used for analysis" []
synonym: "FrtSample_Cnt" EXACT []
namespace: INV
relationship: variable_of INV:0000050 ! Sampled Fruit Number

[Term] 
id: INV:0000173
name: Scion Trunk Diameter - East to West - centimeters
def: "Measurement of scion diameter just above bud union from East to West in cm." []
synonym: "ScionDia_EW_cm" EXACT []
namespace: INV
relationship: variable_of INV:0000051 ! Scion Trunk Diameter

[Term] 
id: INV:0000174
name: Scion Trunk Diameter - East to West Measurement - inches
def: "Measurement of scion diameter just above bud union from East to West in inches." []
synonym: "ScionDia_EW_in" EXACT []
namespace: INV
relationship: variable_of INV:0000051 ! Scion Trunk Diameter

[Term] 
id: INV:0000175
name: Scion Trunk Diameter - North to South - centimeters
def: "Measurement of scion diameter just above bud union from North to South in cm." []
synonym: "ScionDia_NS_cm" EXACT []
namespace: INV
relationship: variable_of INV:0000051 ! Scion Trunk Diameter

[Term] 
id: INV:0000176
name: Scion Trunk Diameter - North to South Measurement - inches
def: "Measurement of scion diameter just above bud union from North to South in inches." []
synonym: "ScionDia_NS_in" EXACT []
namespace: INV
relationship: variable_of INV:0000051 ! Scion Trunk Diameter

[Term] 
id: INV:0000177
name: Seed Count - Sample
def: "Count of all seeds in a fruit sample." []
synonym: "Seed_Cnt" EXACT []
namespace: INV
relationship: variable_of INV:0000052 ! Seed Count

[Term] 
id: INV:0000178
name: Seed Water Loss - Calculation - percentage
def: "Seed water loss calculation as a percentage. WatLoss = (Fresh Weight - Dry Weight)/(Fresh Weight)" []
synonym: "SdWatLoss_Comp_pct" EXACT []
namespace: INV
relationship: variable_of INV:0000053 ! Seed Water Loss

[Term] 
id: INV:0000179
name: Soil Moisture - water fraction by volume
def: "Measurement of soil moisture using a soil moisture probe (wfv)" []
synonym: "SoilMst_wfv" EXACT []
namespace: INV
relationship: variable_of INV:0000054 ! Soil Moisture

[Term] 
id: INV:0000180
name: Soil Moisture Rating - 1-3 Soil Moisture Scale
def: "Estimation of soil moisture using a rating scale." []
synonym: "SoilMst_Rate" EXACT []
namespace: INV
relationship: variable_of INV:0000054 ! Soil Moisture

[Term] 
id: INV:0000181
name: Total Soluble Solids - Degrees Brix
def: "Brix (total soluble solids) measurement in juice from fruit sample with refractometer in degrees Brix." []
synonym: "TSS_dBx; TSS" EXACT []
namespace: INV
relationship: variable_of INV:0000055 ! Total Soluble Solids

[Term] 
id: INV:0000182
name: Tree Yield - Count using Machine Learning
def: "Count of Fruit on Tree using Machine Learning on Image of Tree" []
synonym: "Yield_ML_ct" EXACT []
namespace: INV
relationship: variable_of INV:0000056 ! Tree Yield

[Term] 
id: INV:0000183
name: Tree Yield - Manual - Count
def: "Manual Count of Fruit on Tree" []
synonym: "Yield_Man_ct" EXACT []
namespace: INV
relationship: variable_of INV:0000056 ! Tree Yield

[Term] 
id: INV:0000184
name: Tree Yield - Weight of All Fruit Harvested - kilograms
def: "Weight of all Fruit on Tree Harvested for Yield Estimation in kilograms." []
synonym: "Yield_Wt_kg" EXACT []
namespace: INV
relationship: variable_of INV:0000056 ! Tree Yield

[Term] 
id: INV:0000185
name: Tree Yield - Weight of All Fruit Harvested - pounds
def: "Weight of all Fruit on Tree Harvested for Yield Estimation in pounds." []
synonym: "Yield_Wt_lbs" EXACT []
namespace: INV
relationship: variable_of INV:0000056 ! Tree Yield

[Term] 
id: INV:0000186
name: Turgid Leaf Weight - grams
def: "Leaf sample weight in grams after soaked in distilled water for 3 hours in the dark at room temp." []
synonym: "TrgdLfWt_g" EXACT []
namespace: INV
relationship: variable_of INV:0000057 ! Turgid Leaf Weight

[Term] 
id: INV:0000187
name: Wet Soil Weight - grams
def: "Direct measurement of the weight in grams of a soil sample when freshly collected." []
synonym: "WetSoilWt_g" EXACT []
namespace: INV
relationship: variable_of INV:0000058 ! Wet Soil Weight

[Term] 
id: INV:0000188
name: Germplasm Intake
def: "" []
namespace: INV
is_a: INV:0000004 ! Morphological

[Term] 
id: INV:0000189
name: Propagation Information
def: "" []
namespace: INV
is_a: INV:0000004 ! Morphological

[Term] 
id: INV:0000200
name: Rootstock Name
def: "" []
namespace: INV
is_a: INV:0000004 ! Morphological

[Term] 
id: INV:0000201
name: Explant Size - Categorical
def: "Size of explant used for propagation" []
synonym: "ExplantSize" EXACT []
namespace: INV
relationship: variable_of INV:0000189 ! Propagation Information

[Term] 
id: INV:0000202
name: Germplasm Intake - Type - Categorical
def: "Tissue type of material received from source by repository." []
synonym: "MaterialType" EXACT []
namespace: INV
relationship: variable_of INV:0000188 ! Germplasm Intake

[Term] 
id: INV:0000203
name: Germplasm Intake- Date - YYYY-MM-DD
def: "Date accession/plant/source was received/collected by repository." []
synonym: "MatRcvdDate" EXACT []
namespace: INV
relationship: variable_of INV:0000188 ! Germplasm Intake

[Term] 
id: INV:0000204
name: Propagation Acclimation End - Date
def: "End date for propagation acclimation." []
synonym: "AccEndDate" EXACT []
namespace: INV
relationship: variable_of INV:0000189 ! Propagation Information

[Term] 
id: INV:0000205
name: Propagation Acclimation Initial Settings - Text
def: "Initial setting for propagation acclimation." []
synonym: "PropAccInitial" EXACT []
namespace: INV
relationship: variable_of INV:0000189 ! Propagation Information

[Term] 
id: INV:0000206
name: Propagation Acclimation Start - Date
def: "Start date for propagation acclimation." []
synonym: "AccStrtDate" EXACT []
namespace: INV
relationship: variable_of INV:0000189 ! Propagation Information

[Term] 
id: INV:0000207
name: Propagation Contamination - Categorical
def: "Indicator of the presence of propagation contamination." []
synonym: "PropContam" EXACT []
namespace: INV
relationship: variable_of INV:0000189 ! Propagation Information

[Term] 
id: INV:0000208
name: Propagation Discard Date - YYYY-MM-DD
def: "Date propagation was discarded." []
synonym: "PropDiscardDate" EXACT []
namespace: INV
relationship: variable_of INV:0000189 ! Propagation Information

[Term] 
id: INV:0000209
name: Propagation Discard Reason - Text
def: "Reason for discarding propagation." []
synonym: "PropDiscardRsn" EXACT []
namespace: INV
relationship: variable_of INV:0000189 ! Propagation Information

[Term] 
id: INV:0000210
name: Propagation Experimental Treatment
def: "Experimental treatment applied to propagation for testing." []
synonym: "PropExpTrt" EXACT []
namespace: INV
relationship: variable_of INV:0000189 ! Propagation Information

[Term] 
id: INV:0000211
name: Propagation Explant Type - Categorical
def: "Type of explant used for propagation." []
synonym: "PropExplantType" EXACT []
namespace: INV
relationship: variable_of INV:0000189 ! Propagation Information

[Term] 
id: INV:0000212
name: Propagation Final Location
def: "Propagation Final Location" []
synonym: "PropFinalLoc" EXACT []
namespace: INV
relationship: variable_of INV:0000189 ! Propagation Information

[Term] 
id: INV:0000213
name: Propagation Final Transfer Date - YYYY-MM-DD
def: "Final transfer date for propagation." []
synonym: "FinalTrnsDate" EXACT []
namespace: INV
relationship: variable_of INV:0000189 ! Propagation Information

[Term] 
id: INV:0000214
name: Propagation Growth Chamber Removal - Date
def: "Propagation Growth Chamber Removal Date" []
synonym: "PropGCRmvDate" EXACT []
namespace: INV
relationship: variable_of INV:0000189 ! Propagation Information

[Term] 
id: INV:0000215
name: Propagation Medium Creator - Text
def: "Initials of person who made medium for propagations." []
synonym: "PropMediumCreator" EXACT []
namespace: INV
relationship: variable_of INV:0000189 ! Propagation Information

[Term] 
id: INV:0000216
name: Propagation Medium Date - YYYY-MM-DD
def: "Date medium used for propagation was created" []
synonym: "PropMediumDate" EXACT []
namespace: INV
relationship: variable_of INV:0000189 ! Propagation Information

[Term] 
id: INV:0000217
name: Propagation Medium Type - Text
def: "Type of medium used for propagation." []
synonym: "PropMedium" EXACT []
namespace: INV
relationship: variable_of INV:0000189 ! Propagation Information

[Term] 
id: INV:0000218
name: Propagation Planter - Text
def: "Initials of person who planted propagation." []
synonym: "PropPlanter" EXACT []
namespace: INV
relationship: variable_of INV:0000189 ! Propagation Information

[Term] 
id: INV:0000219
name: Propagation Planting Container - Text
def: "Container used to for planting propagation." []
synonym: "PropPlantContr" EXACT []
namespace: INV
relationship: variable_of INV:0000189 ! Propagation Information

[Term] 
id: INV:0000220
name: Propagation Prep and Disinfestation Protocol
def: "Protocol used to prepare and disinfect tissue for propagation. 1 = Remove seed coats manually, 20 percent bleach for 20 mins., Rinse 3x sterile H2O; 2 = Rinse budwood, cut into nodal segments, water soak 3 hrs, 1 min 70 percent isopropyl alcohol, 20 mins 20 percent bleach, rinse 3x with sterile H2O; 3 = Rinse budwood, cut into 1-2  inch segments, water soak 2 hrs, 1 min 70 percent isopropyl alcohol, 20 mins 20 percent bleach, rinse 3x with sterile H2O, 5 mins 100 percent PPM soak; 4 = CCPP Protocol; 5 = CCPP Protocol without cut ends" []
synonym: "PropPrepDis" EXACT []
namespace: INV
relationship: variable_of INV:0000189 ! Propagation Information

[Term] 
id: INV:0000221
name: Propagation Soil Type - Text
def: "Soil type used for propagation final transplant." []
synonym: "FinTrnsSoilType" EXACT []
namespace: INV
relationship: variable_of INV:0000189 ! Propagation Information

[Term] 
id: INV:0000222
name: Propagation Transfer Date - YYYY-MM-DD
def: "Date propagation was transferred to new medium." []
synonym: "PropTrnsDate" EXACT []
namespace: INV
relationship: variable_of INV:0000189 ! Propagation Information

[Term] 
id: INV:0000223
name: Propagation Vessel - Categorical
def: "Vessel used to store propagation." []
synonym: "PropVessel" EXACT []
namespace: INV
relationship: variable_of INV:0000189 ! Propagation Information

[Term] 
id: INV:0000224
name: Propagator - Categorical
def: "Person who performed propagation." []
synonym: "PropPerson" EXACT []
namespace: INV
relationship: variable_of INV:0000189 ! Propagation Information

[Term] 
id: INV:0000225
name: Rootstock Graft - Text
def: "Name of rootstock used for graft." []
synonym: "RtstckGrft" EXACT []
namespace: INV
relationship: variable_of INV:0000200 ! Rootstock Name

[Term]
id: INV:0000226
name: Fruit Perimeter from Side 1 of Whole Fruit Imaged with Poles Parallel (mm)
def: "Whole fruit is imaged on a single side (side 1) with poles oriented parallel to background surface. The total distance around outer border of fruit is measured in mm" []
synonym: "FrtPermtr_WVS1_mm" EXACT []
namespace: INV
relationship: variable of INV:0000004 ! Morphological

[Term]
id: INV:0000227
name: Fruit Perimeter from Side 2 of Whole Fruit Imaged with Poles Parallel (mm) 
def: "Whole fruit is imaged on side 2 (180 degree rotation from side 1) with poles oriented parallel to background surface. The total distance around outer border of fruit is measured in mm FrtPermtr_WVS2_mm" []
synonym: "FrtPermtr_WVS2_mm" EXACT []
namespace: INV
relationship: variable_of INV:0000004 ! Morphological

[Term]
id: INV:0000228
name: Fruit Perimeter from Side 2 of Whole Fruit Imaged with Poles Perpendicular (mm)
def: "Whole fruit is imaged on a single side (side 1) with poles oriented perpendicular to background surface. The around outer border of fruit is measured in mm" []
synonym: "FrtPermtr_WHS1_mm" EXACT []
namespace: INV
relationship: variable_of INV:0000004 ! Morphological

[Term]
id: INV:0000229
name: Fruit Perimeter from Side 2 of Whole Fruit Imaged with Poles Perpendicular (mm)
def: "Whole fruit is imaged on 2 (180 degree rotation from side 1) with poles oriented perpendicular to background surface. The around outer border of fruit is measured in mm" []
synonym: "FrtPermtr_WHS2_mm" EXACT []
namespace: INV
relationship: variable_of INV:0000004 ! Morphological

[Term]
id: INV:0000230
name: Puff Skin Rating
def: "Rating of the amount of puffy skin observed on date fruit where 1=0-5%, 2=5-25%, 3=25-50%, and 4=>50%" []
synonym: "PuffRate" EXACT []
relationship: variable_of INV:0000004 ! Morphological

[Term]
id: INV:0000231
name: Acidity Measurement
def: "Titration Juice acidity from fruit sample using titration" []
synonym: "Acid_Titration" EXACT []
relationship: variable_of id: INV:0000007 ! Acid


