format-version: 1.2
date: 10:03:2024 17:10
saved-by: Lukas_Mueller
default-namespace: INV
ontology: CO_365


[Term]
id: INV:0000000
name: ROOT
namespace: INV

[Term] 
id: INV:0000001
name: Abiotic Stress
def: "Abiotic Stress" []
namespace: INV
is_a: INV:0000000 ! ROOT

[Term] 
id: INV:0000002
name: Agronomic
def: "Agronomic" []
namespace: INV
is_a: INV:0000000 ! ROOT

[Term] 
id: INV:0000003
name: Biotic Stress
def: "Biotic Stress" []
namespace: INV
is_a: INV:0000000 ! ROOT

[Term] 
id: INV:0000004
name: Morphological
def: "Morphological" []
namespace: INV
is_a: INV:0000000 ! ROOT

[Term] 
id: INV:0000005
name: Physiological
def: "Physiological" []
namespace: INV
is_a: INV:0000000 ! ROOT

[Term] 
id: INV:0000006
name: Quality
def: "Quality" []
namespace: INV
is_a: INV:0000000 ! ROOT

[Term] 
id: INV:0000007
name: Acid
def: "" []
namespace: INV
is_a: INV:0000006 ! Quality

[Term] 
id: INV:0000008
name: Biological Index Inoculation Date
def: "" []
namespace: INV
is_a: INV:0000003 ! Biotic Stress

[Term] 
id: INV:0000009
name: Biological Index Inoculation Source Tree
def: "" []
namespace: INV
is_a: INV:0000003 ! Biotic Stress

[Term] 
id: INV:0000010
name: Biological Index Result
def: "" []
namespace: INV
is_a: INV:0000003 ! Biotic Stress

[Term] 
id: INV:0000011
name: Brix Acid Ratio
def: "" []
namespace: INV
is_a: INV:0000006 ! Quality

[Term] 
id: INV:0000012
name: Canopy Color
def: "" []
namespace: INV
is_a: INV:0000004 ! Morphological

[Term] 
id: INV:0000013
name: Canopy Density
def: "" []
namespace: INV
is_a: INV:0000004 ! Morphological

[Term] 
id: INV:0000014
name: Canopy Diameter
def: "" []
namespace: INV
is_a: INV:0000004 ! Morphological

[Term] 
id: INV:0000015
name: Canopy Volume
def: "" []
namespace: INV
is_a: INV:0000004 ! Morphological

[Term] 
id: INV:0000016
name: Chopped Fruit Weight
def: "" []
namespace: INV
is_a: INV:0000004 ! Morphological

[Term] 
id: INV:0000017
name: Days to Recover
def: "" []
namespace: INV
is_a: INV:0000001 ! Abiotic Stress

[Term] 
id: INV:0000018
name: Days to Wilt
def: "" []
namespace: INV
is_a: INV:0000001 ! Abiotic Stress

[Term] 
id: INV:0000019
name: Dry Fruit Weight
def: "" []
namespace: INV
is_a: INV:0000004 ! Morphological

[Term] 
id: INV:0000020
name: Dry Leaf Weight
def: "" []
namespace: INV
is_a: INV:0000004 ! Morphological

[Term] 
id: INV:0000021
name: Dry Seed Weight
def: "" []
namespace: INV
is_a: INV:0000004 ! Morphological

[Term] 
id: INV:0000022
name: Dry Soil Weight
def: "" []
namespace: INV
is_a: INV:0000001 ! Abiotic Stress

[Term] 
id: INV:0000023
name: Endocarp Color
def: "" []
namespace: INV
is_a: INV:0000004 ! Morphological

[Term] 
id: INV:0000024
name: Exocarp Color
def: "" []
namespace: INV
is_a: INV:0000004 ! Morphological

[Term] 
id: INV:0000025
name: Exocarp Texture
def: "" []
namespace: INV
is_a: INV:0000004 ! Morphological

[Term] 
id: INV:0000026
name: Exocarp Thickness
def: "" []
namespace: INV
is_a: INV:0000004 ! Morphological

[Term] 
id: INV:0000027
name: Final Fruit Temperature
def: "" []
namespace: INV
is_a: INV:0000005 ! Physiological

[Term] 
id: INV:0000028
name: Fresh Fruit Weight
def: "" []
namespace: INV
is_a: INV:0000004 ! Morphological

[Term] 
id: INV:0000029
name: Fresh Leaf Weight
def: "" []
namespace: INV
is_a: INV:0000004 ! Morphological

[Term] 
id: INV:0000030
name: Fresh Seed Weight
def: "" []
namespace: INV
is_a: INV:0000004 ! Morphological

[Term] 
id: INV:0000031
name: Fruit Area
def: "" []
namespace: INV
is_a: INV:0000004 ! Morphological

[Term] 
id: INV:0000032
name: Fruit Collection Date
def: "" []
namespace: INV
is_a: INV:0000004 ! Morphological

[Term] 
id: INV:0000033
name: Fruit Diameter
def: "" []
namespace: INV
is_a: INV:0000004 ! Morphological

[Term] 
id: INV:0000034
name: Fruit Longest Path
def: "" []
namespace: INV
is_a: INV:0000004 ! Morphological

[Term] 
id: INV:0000035
name: Fruit Perimeter
def: "" []
namespace: INV
is_a: INV:0000004 ! Morphological

[Term] 
id: INV:0000036
name: Fruit Volume
def: "" []
namespace: INV
is_a: INV:0000004 ! Morphological

[Term] 
id: INV:0000037
name: Fruit Water Activity
def: "" []
namespace: INV
is_a: INV:0000005 ! Physiological

[Term] 
id: INV:0000038
name: Fruit Water Loss
def: "" []
namespace: INV
is_a: INV:0000001 ! Abiotic Stress

[Term] 
id: INV:0000039
name: Fruit Water Potential
def: "" []
namespace: INV
is_a: INV:0000005 ! Physiological

[Term] 
id: INV:0000040
name: Graft Survival
def: "" []
namespace: INV
is_a: INV:0000002 ! Agronomic

[Term] 
id: INV:0000041
name: Graft Survival Date
def: "" []
namespace: INV
is_a: INV:0000002 ! Agronomic

[Term] 
id: INV:0000042
name: Juice Percent
def: "" []
namespace: INV
is_a: INV:0000006 ! Quality

[Term] 
id: INV:0000043
name: Juice Weight
def: "" []
namespace: INV
is_a: INV:0000002 ! Agronomic

[Term] 
id: INV:0000044
name: Leaf Collection Date
def: "" []
namespace: INV
is_a: INV:0000004 ! Morphological

[Term] 
id: INV:0000045
name: Leaf Conductance
def: "" []
namespace: INV
is_a: INV:0000005 ! Physiological

[Term] 
id: INV:0000046
name: Leaf Relative Humidity
def: "" []
namespace: INV
is_a: INV:0000005 ! Physiological

[Term] 
id: INV:0000047
name: Leaf Relative Water Content
def: "" []
namespace: INV
is_a: INV:0000005 ! Physiological

[Term] 
id: INV:0000048
name: Leaf Water Loss
def: "" []
namespace: INV
is_a: INV:0000001 ! Abiotic Stress

[Term] 
id: INV:0000049
name: Rootstock Trunk Diameter
def: "" []
namespace: INV
is_a: INV:0000004 ! Morphological

[Term] 
id: INV:0000050
name: Sampled Fruit Number
def: "" []
namespace: INV
is_a: INV:0000002 ! Agronomic

[Term] 
id: INV:0000051
name: Scion Trunk Diameter
def: "" []
namespace: INV
is_a: INV:0000004 ! Morphological

[Term] 
id: INV:0000052
name: Seed Count
def: "" []
namespace: INV
is_a: INV:0000006 ! Quality

[Term] 
id: INV:0000053
name: Seed Water Loss
def: "" []
namespace: INV
is_a: INV:0000001 ! Abiotic Stress

[Term] 
id: INV:0000054
name: Soil Moisture
def: "" []
namespace: INV
is_a: INV:0000001 ! Abiotic Stress

[Term] 
id: INV:0000055
name: Total Soluble Solids
def: "" []
namespace: INV
is_a: INV:0000006 ! Quality

[Term] 
id: INV:0000056
name: Tree Yield
def: "" []
namespace: INV
is_a: INV:0000002 ! Agronomic

[Term] 
id: INV:0000057
name: Turgid Leaf Weight
def: "" []
namespace: INV
is_a: INV:0000004 ! Morphological

[Term] 
id: INV:0000058
name: Wet Soil Weight
def: "" []
namespace: INV
is_a: INV:0000001 ! Abiotic Stress

[Term] 
id: INV:0000059
name: Acid - Acidity Measurement - no unit
def: "Juice acidity from fruit sample using titration." []
namespace: INV
relationship: variable_of INV:0000007 ! Acid

[Term] 
id: INV:0000060
name: Biological Index Inoculation Date - Biological Index Inoculation Date - YYYY-MM-DD
def: "Date tree was inoculated with pathogen for bioindexing" []
namespace: INV
relationship: variable_of INV:0000008 ! Biological Index Inoculation Date

[Term] 
id: INV:0000061
name: Biological Index Inoculation Source Tree - Biological Index Inoculation Source Tree - Free Text
def: "Unique identifier of positive source tree used for inoculation." []
namespace: INV
relationship: variable_of INV:0000009 ! Biological Index Inoculation Source Tree

[Term] 
id: INV:0000062
name: Biological Index Result - Biological Index Result - 0-11 Bioindex Result Scale
def: "Visual estimation of bioindexing result" []
namespace: INV
relationship: variable_of INV:0000010 ! Biological Index Result

[Term] 
id: INV:0000063
name: Brix Acid Ratio - Calculation of Brix Acid Ratio - no unit
def: "Brix/TSS measurement divided by Titratable Acidity Measurement" []
namespace: INV
relationship: variable_of INV:0000011 ! Brix Acid Ratio

[Term] 
id: INV:0000064
name: Canopy Color - Canopy Color Rating - 1-5 Canopy Color Rating
def: "Rating of overall color of canopy from 1 to 5, where 1=very yellow, worst and 5=very green, best." []
namespace: INV
relationship: variable_of INV:0000012 ! Canopy Color

[Term] 
id: INV:0000065
name: Canopy Density - Canopy Density with Digital Canopy Analyzer Measurement - LAI
def: "Tree Canopy Density Measurement using Digital Canopy Analyzer" []
namespace: INV
relationship: variable_of INV:0000013 ! Canopy Density

[Term] 
id: INV:0000066
name: Canopy Diameter - Canopy Width/Diameter from East to West Measurement - centimeters
def: "Canopy width measurement from East to West in cm." []
namespace: INV
relationship: variable_of INV:0000014 ! Canopy Diameter

[Term] 
id: INV:0000067
name: Canopy Diameter - Canopy Width/Diameter from North to South Measurement - centimeters
def: "Canopy width measurement from North to South in cm." []
namespace: INV
relationship: variable_of INV:0000014 ! Canopy Diameter

[Term] 
id: INV:0000068
name: Canopy Volume - Canopy Volume Calculation - m^3
def: "Calculation of canopy volume based on Canopy Diameter from N-S, Canopy Diameter from E-W, and Height of Tree. (NS_Dia*EW_Dia*TreeHt)/4" []
namespace: INV
relationship: variable_of INV:0000015 ! Canopy Volume

[Term] 
id: INV:0000069
name: Chopped Fruit Weight - Chopped Fruit Weight Measurement - grams
def: "Fruit sample weight after chopping for evaluation  in grams." []
namespace: INV
relationship: variable_of INV:0000016 ! Chopped Fruit Weight

[Term] 
id: INV:0000070
name: Days to Recover - Days to Recovery - count
def: "A count of the number of days after water reintroduction until tree recovers." []
namespace: INV
relationship: variable_of INV:0000017 ! Days to Recover

[Term] 
id: INV:0000071
name: Days to Wilt - Days to Wilt - count
def: "A count of the number of days after drought conditions are applied until tree wilts." []
namespace: INV
relationship: variable_of INV:0000018 ! Days to Wilt

[Term] 
id: INV:0000072
name: Dry Fruit Weight - Dry Fruit Weight Measurement - grams
def: "Fruit sample weight after drying in grams." []
namespace: INV
relationship: variable_of INV:0000019 ! Dry Fruit Weight

[Term] 
id: INV:0000073
name: Dry Leaf Weight - Dry Leaf Tissue Weight Measurement - grams
def: "Leaf sample weight in grams after drying in oven at 85C overnight" []
namespace: INV
relationship: variable_of INV:0000020 ! Dry Leaf Weight

[Term] 
id: INV:0000074
name: Dry Seed Weight - Dry Seed Weight Measurement - grams
def: "Seed sample weight in grams after drying." []
namespace: INV
relationship: variable_of INV:0000021 ! Dry Seed Weight

[Term] 
id: INV:0000075
name: Dry Soil Weight - Dry Soil Weight Measurement - grams
def: "Direct measurement of the weight of a soil sample after drying." []
namespace: INV
relationship: variable_of INV:0000022 ! Dry Soil Weight

[Term] 
id: INV:0000076
name: Endocarp Color - Class 1 Color Percentage - percentage
def: "Percentage of pixels assigned to class 1 color bin (RGB 173 90 32) using Naïve Bayes. (# Assigned Pixels)/(Total # Pixels)" []
namespace: INV
relationship: variable_of INV:0000023 ! Endocarp Color

[Term] 
id: INV:0000077
name: Endocarp Color - Class 1 Color Pixel Count - count
def: "Number of pixels assigned to class 1 color bin (RGB 173 90 32) using Naïve Bayes." []
namespace: INV
relationship: variable_of INV:0000023 ! Endocarp Color

[Term] 
id: INV:0000078
name: Endocarp Color - Class 10 Color Percentage - percentage
def: "Percentage of pixels assigned to class 10 color bin (RGB 173 90 32) using Naïve Bayes. (# Assigned Pixels)/(Total # Pixels)" []
namespace: INV
relationship: variable_of INV:0000023 ! Endocarp Color

[Term] 
id: INV:0000079
name: Endocarp Color - Class 10 Color Pixel Count - count
def: "Number of pixels assigned to class 10 color bin (RGB 173 90 32) using Naïve Bayes." []
namespace: INV
relationship: variable_of INV:0000023 ! Endocarp Color

[Term] 
id: INV:0000080
name: Endocarp Color - Class 2 Color Percentage - percentage
def: "Percentage of pixels assigned to class 2 color bin (RGB 173 90 32) using Naïve Bayes. (# Assigned Pixels)/(Total # Pixels)" []
namespace: INV
relationship: variable_of INV:0000023 ! Endocarp Color

[Term] 
id: INV:0000081
name: Endocarp Color - Class 2 Color Pixel Count - count
def: "Number of pixels assigned to class 2 color bin (RGB 173 90 32) using Naïve Bayes." []
namespace: INV
relationship: variable_of INV:0000023 ! Endocarp Color

[Term] 
id: INV:0000082
name: Endocarp Color - Class 3 Color Percentage - percentage
def: "Percentage of pixels assigned to class 3 color bin (RGB 173 90 32) using Naïve Bayes. (# Assigned Pixels)/(Total # Pixels)" []
namespace: INV
relationship: variable_of INV:0000023 ! Endocarp Color

[Term] 
id: INV:0000083
name: Endocarp Color - Class 3 Color Pixel Count - count
def: "Number of pixels assigned to class 3 color bin (RGB 173 90 32) using Naïve Bayes." []
namespace: INV
relationship: variable_of INV:0000023 ! Endocarp Color

[Term] 
id: INV:0000084
name: Endocarp Color - Class 6 Color Percentage - percentage
def: "Percentage of pixels assigned to class 6 color bin (RGB 173 90 32) using Naïve Bayes. (# Assigned Pixels)/(Total # Pixels)" []
namespace: INV
relationship: variable_of INV:0000023 ! Endocarp Color

[Term] 
id: INV:0000085
name: Endocarp Color - Class 6 Color Pixel Count - count
def: "Number of pixels assigned to class 6 color bin (RGB 173 90 32) using Naïve Bayes." []
namespace: INV
relationship: variable_of INV:0000023 ! Endocarp Color

[Term] 
id: INV:0000086
name: Endocarp Color - Class 8 Color Percentage - percentage
def: "Percentage of pixels assigned to class 8 color bin (RGB 173 90 32) using Naïve Bayes. (# Assigned Pixels)/(Total # Pixels)" []
namespace: INV
relationship: variable_of INV:0000023 ! Endocarp Color

[Term] 
id: INV:0000087
name: Endocarp Color - Class 8 Color Pixel Count - count
def: "Number of pixels assigned to class 8 color bin (RGB 173 90 32) using Naïve Bayes." []
namespace: INV
relationship: variable_of INV:0000023 ! Endocarp Color

[Term] 
id: INV:0000088
name: Endocarp Color - Endocarp Color Rating - 0-7 Endocarp Fruit Color Scale
def: "Estimation of endocarp color using a rating scale" []
namespace: INV
relationship: variable_of INV:0000023 ! Endocarp Color

[Term] 
id: INV:0000089
name: Exocarp Color - Class 1 Color Percentage - percentage
def: "Percentage of pixels assigned to class 1 color bin (RGB 173 90 32) using Naïve Bayes. (# Assigned Pixels)/(Total # Pixels)" []
namespace: INV
relationship: variable_of INV:0000024 ! Exocarp Color

[Term] 
id: INV:0000090
name: Exocarp Color - Class 1 Color Pixel Count - count
def: "Number of pixels assigned to class 1 color bin (RGB 173 90 32) using Naïve Bayes." []
namespace: INV
relationship: variable_of INV:0000024 ! Exocarp Color

[Term] 
id: INV:0000091
name: Exocarp Color - Class 10 Color Percentage - percentage
def: "Percentage of pixels assigned to class 10 color bin (RGB 173 90 32) using Naïve Bayes. (# Assigned Pixels)/(Total # Pixels)" []
namespace: INV
relationship: variable_of INV:0000024 ! Exocarp Color

[Term] 
id: INV:0000092
name: Exocarp Color - Class 10 Color Pixel Count - count
def: "Number of pixels assigned to class 10 color bin (RGB 173 90 32) using Naïve Bayes." []
namespace: INV
relationship: variable_of INV:0000024 ! Exocarp Color

[Term] 
id: INV:0000093
name: Exocarp Color - Class 2 Color Percentage - percentage
def: "Percentage of pixels assigned to class 2 color bin (RGB 173 90 32) using Naïve Bayes. (# Assigned Pixels)/(Total # Pixels)" []
namespace: INV
relationship: variable_of INV:0000024 ! Exocarp Color

[Term] 
id: INV:0000094
name: Exocarp Color - Class 2 Color Pixel Count - count
def: "Number of pixels assigned to class 2 color bin (RGB 173 90 32) using Naïve Bayes." []
namespace: INV
relationship: variable_of INV:0000024 ! Exocarp Color

[Term] 
id: INV:0000095
name: Exocarp Color - Class 3 Color Percentage - percentage
def: "Percentage of pixels assigned to class 3 color bin (RGB 173 90 32) using Naïve Bayes. (# Assigned Pixels)/(Total # Pixels)" []
namespace: INV
relationship: variable_of INV:0000024 ! Exocarp Color

[Term] 
id: INV:0000096
name: Exocarp Color - Class 3 Color Pixel Count - count
def: "Number of pixels assigned to class 3 color bin (RGB 173 90 32) using Naïve Bayes." []
namespace: INV
relationship: variable_of INV:0000024 ! Exocarp Color

[Term] 
id: INV:0000097
name: Exocarp Color - Class 6 Color Percentage - percentage
def: "Percentage of pixels assigned to class 6 color bin (RGB 173 90 32) using Naïve Bayes. (# Assigned Pixels)/(Total # Pixels)" []
namespace: INV
relationship: variable_of INV:0000024 ! Exocarp Color

[Term] 
id: INV:0000098
name: Exocarp Color - Class 6 Color Pixel Count - count
def: "Number of pixels assigned to class 6 color bin (RGB 173 90 32) using Naïve Bayes." []
namespace: INV
relationship: variable_of INV:0000024 ! Exocarp Color

[Term] 
id: INV:0000099
name: Exocarp Color - Class 8 Color Percentage - percentage
def: "Percentage of pixels assigned to class 8 color bin (RGB 173 90 32) using Naïve Bayes. (# Assigned Pixels)/(Total # Pixels)" []
namespace: INV
relationship: variable_of INV:0000024 ! Exocarp Color

[Term] 
id: INV:0000100
name: Exocarp Color - Class 8 Color Pixel Count - count
def: "Number of pixels assigned to class 8 color bin (RGB 173 90 32) using Naïve Bayes." []
namespace: INV
relationship: variable_of INV:0000024 ! Exocarp Color

[Term] 
id: INV:0000101
name: Exocarp Color - Exocarp Color Rating - 3-13 Exocarp Fruit Color Scale
def: "Rating of exocarp color based on color reference chart from 3 to 13, where 3 = Dark Green, 5 = Color Break, and 13 = Orange Red." []
namespace: INV
relationship: variable_of INV:0000024 ! Exocarp Color

[Term] 
id: INV:0000102
name: Exocarp Texture - Exocarp Texture Rating - 1-8 Exocarp Texture Scale
def: "Exocarp texture estimation of fruit sample using a rating scale from 1 to 8, where 1 = Smooth and 8 = Rough." []
namespace: INV
relationship: variable_of INV:0000025 ! Exocarp Texture

[Term] 
id: INV:0000103
name: Exocarp Thickness - Exocarp Thickness Measurement - millimeters
def: "Exocarp (rind) thickness in mm of a single fruit." []
namespace: INV
relationship: variable_of INV:0000026 ! Exocarp Thickness

[Term] 
id: INV:0000104
name: Final Fruit Temperature - Aqualab 4TE Final Fruit Temperature Measurement - Degrees Celsius
def: "Final fruit temperature using the Aqualab 4TE meter." []
namespace: INV
relationship: variable_of INV:0000027 ! Final Fruit Temperature

[Term] 
id: INV:0000105
name: Final Fruit Temperature - WP4C Final Fruit Temperature Measurement - Degrees Celsius
def: "Final fruit temperature using the WP4C Dewpoint PotentiaMeter." []
namespace: INV
relationship: variable_of INV:0000027 ! Final Fruit Temperature

[Term] 
id: INV:0000106
name: Fresh Fruit Weight - Fresh Fruit Weight Measurement - grams
def: "Weight of all fruit in sample in grams." []
namespace: INV
relationship: variable_of INV:0000028 ! Fresh Fruit Weight

[Term] 
id: INV:0000107
name: Fresh Fruit Weight - Fresh Fruit Weight Measurement - kilograms
def: "Weight of all fruit in sample in kilograms." []
namespace: INV
relationship: variable_of INV:0000028 ! Fresh Fruit Weight

[Term] 
id: INV:0000108
name: Fresh Leaf Weight - Fresh Leaf Tissue Weight Measurement - grams
def: "Fresh leaf sample weight in grams." []
namespace: INV
relationship: variable_of INV:0000029 ! Fresh Leaf Weight

[Term] 
id: INV:0000109
name: Fresh Seed Weight - Fresh Seed Weight Measurement - grams
def: "Fresh seed sample weight in grams." []
namespace: INV
relationship: variable_of INV:0000030 ! Fresh Seed Weight

[Term] 
id: INV:0000110
name: Fruit Area - Area of Convex Hull of Fruit from Cut Side Down Image Measurement - mm^2
def: "Fruit is cut in half and imaged cut side down. A convex hull is fitted on fruit and area is measured." []
namespace: INV
relationship: variable_of INV:0000031 ! Fruit Area

[Term] 
id: INV:0000111
name: Fruit Area - Area of Convex Hull of Fruit from Cut Side Up Image Measurement - mm^2
def: "Fruit is cut in half and imaged cut side up. A convex hull is fitted on fruit and area is measured." []
namespace: INV
relationship: variable_of INV:0000031 ! Fruit Area

[Term] 
id: INV:0000112
name: Fruit Area - Area of Fruit from Cut Side Down Image Measurement - mm^2
def: "Fruit is cut in half and imaged cut side down and area of entire surface is measured." []
namespace: INV
relationship: variable_of INV:0000031 ! Fruit Area

[Term] 
id: INV:0000113
name: Fruit Area - Area of Fruit from Cut Side Up Image Measurement - mm^2
def: "Fruit is cut in half and imaged cut side up and area of entire surface is measured." []
namespace: INV
relationship: variable_of INV:0000031 ! Fruit Area

[Term] 
id: INV:0000114
name: Fruit Collection Date - Fruit Collection Date - YYYY-MM-DD
def: "Date fruit sample was collected." []
namespace: INV
relationship: variable_of INV:0000032 ! Fruit Collection Date

[Term] 
id: INV:0000115
name: Fruit Diameter - Ellipse Major Axis from Cut Side Down Fruit Image Measurement - millimeters
def: "Fruit is cut in half and imaged cut side down. An ellipse is fitted to fruit and the length of the major axis of ellipse is measured." []
namespace: INV
relationship: variable_of INV:0000033 ! Fruit Diameter

[Term] 
id: INV:0000116
name: Fruit Diameter - Ellipse Major Axis from Cut Side Up Fruit Image Measurement - millimeters
def: "Fruit is cut in half and imaged cut side up. An ellipse is fitted to fruit and the length of the major axis of ellipse is measured." []
namespace: INV
relationship: variable_of INV:0000033 ! Fruit Diameter

[Term] 
id: INV:0000117
name: Fruit Diameter - Ellipse Major Axis from Side 1 of Whole Fruit Imaged with Poles Parallel Measurement - millimeters
def: "Whole fruit is imaged on a single side (side 1) with poles oriented parallel to background surface. An ellipse is fitted to fruit and the length of the major axis of ellipse is measured." []
namespace: INV
relationship: variable_of INV:0000033 ! Fruit Diameter

[Term] 
id: INV:0000118
name: Fruit Diameter - Ellipse Major Axis from Side 1 of Whole Fruit Imaged with Poles Perpendicular Measurement - millimeters
def: "Whole fruit is imaged on a single side (side 1) with poles oriented perpendicular to background surface. An ellipse is fitted to fruit and the length of the major axis of ellipse is measured." []
namespace: INV
relationship: variable_of INV:0000033 ! Fruit Diameter

[Term] 
id: INV:0000119
name: Fruit Diameter - Ellipse Major Axis from Side 2 of Whole Fruit Imaged with Poles Parallel Measurement - millimeters
def: "Whole fruit is imaged on side 2 (180 degree rotation from side 1) with poles oriented parallel to background surface. An ellipse is fitted to fruit and the length of the major axis of ellipse is measured." []
namespace: INV
relationship: variable_of INV:0000033 ! Fruit Diameter

[Term] 
id: INV:0000120
name: Fruit Diameter - Ellipse Major Axis from Side 2 of Whole Fruit Imaged with Poles Perpendicular Measurement - millimeters
def: "Whole fruit is imaged on side 2 (180 degree rotation from side 1) with poles oriented perpendicular to background surface. An ellipse is fitted to fruit and the length of the major axis of ellipse is measured." []
namespace: INV
relationship: variable_of INV:0000033 ! Fruit Diameter

[Term] 
id: INV:0000121
name: Fruit Diameter - Ellipse Minor Axis from Cut Side Down Fruit Image Measurement - millimeters
def: "Fruit is cut in half and imaged cut side down. An ellipse is fitted to fruit and the length of the minor axis of ellipse is measured." []
namespace: INV
relationship: variable_of INV:0000033 ! Fruit Diameter

[Term] 
id: INV:0000122
name: Fruit Diameter - Ellipse Minor Axis from Cut Side Up Fruit Image Measurement - millimeters
def: "Fruit is cut in half and imaged cut side up. An ellipse is fitted to fruit and the length of the minor axis of ellipse is measured." []
namespace: INV
relationship: variable_of INV:0000033 ! Fruit Diameter

[Term] 
id: INV:0000123
name: Fruit Diameter - Ellipse Minor Axis from Side 1 of Whole Fruit Imaged with Poles Parallel Measurement - millimeters
def: "Whole fruit is imaged on a single side (side 1) with oriented parallel to background surface. An ellipse is fitted to fruit and the length of the minor axis of ellipse is measured." []
namespace: INV
relationship: variable_of INV:0000033 ! Fruit Diameter

[Term] 
id: INV:0000124
name: Fruit Diameter - Ellipse Minor Axis from Side 1 of Whole Fruit Imaged with Poles Perpendicular Measurement - millimeters
def: "Whole fruit is imaged on a single side (side 1) with poles oriented perpendicular to background surface. An ellipse is fitted to fruit and the length of the minor axis of ellipse is measured." []
namespace: INV
relationship: variable_of INV:0000033 ! Fruit Diameter

[Term] 
id: INV:0000125
name: Fruit Diameter - Ellipse Minor Axis from Side 2 of Whole Fruit Imaged with Poles Parallel Measurement - millimeters
def: "Whole fruit is imaged on side 2 (180 degree rotation from side 1) with poles oriented parallel to background surface. An ellipse is fitted to fruit and the length of the minor axis of ellipse is measured." []
namespace: INV
relationship: variable_of INV:0000033 ! Fruit Diameter

[Term] 
id: INV:0000126
name: Fruit Diameter - Ellipse Minor Axis from Side 2 of Whole Fruit Imaged with Poles Perpendicular Measurement - millimeters
def: "Whole fruit is imaged on side 2 (180 degree rotation from side 1) with poles oriented perpendicular to background surface. An ellipse is fitted to fruit and the length of the minor axis of ellipse is measured." []
namespace: INV
relationship: variable_of INV:0000033 ! Fruit Diameter

[Term] 
id: INV:0000127
name: Fruit Diameter - Fruit Equatorial Diameter Measurement - millimeters
def: "Equatorial diameter of fruit sample in mm." []
namespace: INV
relationship: variable_of INV:0000033 ! Fruit Diameter

[Term] 
id: INV:0000128
name: Fruit Diameter - Height from Cut Side Down Fruit Image Measurement - millimeters
def: "Fruit is cut in half and imaged cut side down. The verticle axis (height) is measured from furthest point on top and furthest point on bottom of fruit." []
namespace: INV
relationship: variable_of INV:0000033 ! Fruit Diameter

[Term] 
id: INV:0000129
name: Fruit Diameter - Height from Cut Side Up Fruit Image Measurement - millimeters
def: "Fruit is cut in half and imaged cut side up. The verticle axis (height) is measured from furthest point on top and furthest point on bottom of fruit." []
namespace: INV
relationship: variable_of INV:0000033 ! Fruit Diameter

[Term] 
id: INV:0000130
name: Fruit Diameter - Height from Side 1 of Whole Fruit Imaged with Poles Parallel Measurement - millimeters
def: "Whole fruit is imaged on a single side (side 1) with poles oriented parallel to background surface. The verticle axis (height) is measured from furthest point on top and furthest point on bottom of fruit." []
namespace: INV
relationship: variable_of INV:0000033 ! Fruit Diameter

[Term] 
id: INV:0000131
name: Fruit Diameter - Height from Side 1 of Whole Fruit Imaged with Poles Perpendicular Measurement - millimeters
def: "Whole fruit is imaged on a single side (side 1) with poles oriented perpendicular to background surface. The verticle axis (height) is measured from furthest point on top and furthest point on bottom of fruit." []
namespace: INV
relationship: variable_of INV:0000033 ! Fruit Diameter

[Term] 
id: INV:0000132
name: Fruit Diameter - Height from Side 2 of Whole Fruit Imaged with Poles Parallel Measurement - millimeters
def: "Whole fruit is imaged on side 2 (180 degree rotation from side 1) with poles oriented parallel to background surface. The verticle axis (height) is measured from furthest point on top and furthest point on bottom of fruit." []
namespace: INV
relationship: variable_of INV:0000033 ! Fruit Diameter

[Term] 
id: INV:0000133
name: Fruit Diameter - Height from Side 2 of Whole Fruit Imaged with Poles Perpendicular Measurement - millimeters
def: "Whole fruit is imaged on side 2 (180 degree rotation from side 1) with poles oriented perpendicular to background surface. The verticle axis (height) is measured from furthest point on top and furthest point on bottom of fruit." []
namespace: INV
relationship: variable_of INV:0000033 ! Fruit Diameter

[Term] 
id: INV:0000134
name: Fruit Diameter - Manual Fruit Equatorial Diameter Measurement - centimeters
def: "Equatorial diameter of fruit sample in cm." []
namespace: INV
relationship: variable_of INV:0000033 ! Fruit Diameter

[Term] 
id: INV:0000135
name: Fruit Diameter - Manual Fruit Polar Diameter Measurement - centimeters
def: "Polar diameter of single fruit in cm." []
namespace: INV
relationship: variable_of INV:0000033 ! Fruit Diameter

[Term] 
id: INV:0000136
name: Fruit Diameter - Manual Fruit Polar Diameter Measurement - millimeters
def: "Polar diameter of single fruit in mm." []
namespace: INV
relationship: variable_of INV:0000033 ! Fruit Diameter

[Term] 
id: INV:0000137
name: Fruit Diameter - Manual Measurement of Total Width of All Fruit Sampled - centimeters
def: "Measurement of the total length of all fruit (polar diameter) in sample when lined up top-to-bottom" []
namespace: INV
relationship: variable_of INV:0000033 ! Fruit Diameter

[Term] 
id: INV:0000138
name: Fruit Diameter - Width from Cut Side Down Fruit Image Measurement - millimeters
def: "Fruit is cut in half and imaged cut side down. The horizontal axis (width) is measured from furthest point on left and furthest point on right of fruit." []
namespace: INV
relationship: variable_of INV:0000033 ! Fruit Diameter

[Term] 
id: INV:0000139
name: Fruit Diameter - Width from Cut Side Up Fruit Image Measurement - millimeters
def: "Fruit is cut in half and imaged cut side up. The horizontal axis (width) is measured from furthest point on left and furthest point on right of fruit." []
namespace: INV
relationship: variable_of INV:0000033 ! Fruit Diameter

[Term] 
id: INV:0000140
name: Fruit Diameter - Width from Side 1 of Whole Fruit Imaged with Poles Parallel Measurement - millimeters
def: "Whole fruit is imaged on a single side (side 1) with poles oriented parallel to background surface. The horizontal axis (width) is measured from furthest point on left and furthest point on right of fruit." []
namespace: INV
relationship: variable_of INV:0000033 ! Fruit Diameter

[Term] 
id: INV:0000141
name: Fruit Diameter - Width from Side 1 of Whole Fruit Imaged with Poles Perpendicular Measurement - millimeters
def: "Whole fruit is imaged on a single side (side 1) with poles oriented perpendicular to background surface. The horizontal axis (width) is measured from furthest point on left and furthest point on right of fruit." []
namespace: INV
relationship: variable_of INV:0000033 ! Fruit Diameter

[Term] 
id: INV:0000142
name: Fruit Diameter - Width from Side 2 of Whole Fruit Imaged with Poles Parallel Measurement - millimeters
def: "Whole fruit is imaged on side 2 (180 degree rotation from side 1) with poles oriented parallel to background surface. The horizontal axis (width) is measured from furthest point on left and furthest point on right of fruit." []
namespace: INV
relationship: variable_of INV:0000033 ! Fruit Diameter

[Term] 
id: INV:0000143
name: Fruit Diameter - Width from Side 2 of Whole Fruit Imaged with Poles Perpendicular Measurement - millimeters
def: "Whole fruit is imaged on side 2 (180 degree rotation from side 1) with poles oriented perpendicular to background surface. The horizontal axis (width) is measured from furthest point on left and furthest point on right of fruit." []
namespace: INV
relationship: variable_of INV:0000033 ! Fruit Diameter

[Term] 
id: INV:0000144
name: Fruit Longest Path - The longest path through fruit imaged Cut Side Down Measurement - millimeters
def: "Fruit is cut in half and imaged cut side down and the length of the line through center of mass and furthest point on the convex hull around fruit is measured." []
namespace: INV
relationship: variable_of INV:0000034 ! Fruit Longest Path

[Term] 
id: INV:0000145
name: Fruit Longest Path - The longest path through fruit imaged Cut Side Up Measurement - millimeters
def: "Fruit is cut in half and imaged cut side up and the length of the line through center of mass and furthest point on the convex hull around fruit is measured." []
namespace: INV
relationship: variable_of INV:0000034 ! Fruit Longest Path

[Term] 
id: INV:0000146
name: Fruit Perimeter - Perimeter of fruit from Cut Side Down Image Measurement - millimeters
def: "Fruit is cut in half and imaged cut side down. The perimeter around outer edge of fruit is measured." []
namespace: INV
relationship: variable_of INV:0000035 ! Fruit Perimeter

[Term] 
id: INV:0000147
name: Fruit Perimeter - Perimeter of fruit from Cut Side Up Image Measurement - millimeters
def: "Fruit is cut in half and imaged cut side up. The perimeter around outer edge of fruit is measured." []
namespace: INV
relationship: variable_of INV:0000035 ! Fruit Perimeter

[Term] 
id: INV:0000148
name: Fruit Volume - Fruit volume calculation of fruit using major axis of ellipse from Cut Side Down image - mm^3
def: "Fruit is cut in half and imaged cut side down. Volume is calculated based on major axis of the fitted ellipse (V=(Ï€d^3)/6)" []
namespace: INV
relationship: variable_of INV:0000036 ! Fruit Volume

[Term] 
id: INV:0000149
name: Fruit Volume - Fruit volume calculation of fruit using major axis of ellipse from Cut Side Up image - mm^3
def: "Fruit is cut in half and imaged cut side down. Volume is calculated based on minor axis of the fitted ellipse (V=(Ï€d^3)/6)" []
namespace: INV
relationship: variable_of INV:0000036 ! Fruit Volume

[Term] 
id: INV:0000150
name: Fruit Volume - Volume of fruit calculation using major axis of ellipse from Cut Side Up Image - mm^3
def: "Fruit is cut in half and imaged cut side up. Volume is calculated based on major axis of the fitted ellipse (V=(Ï€d^3)/6)" []
namespace: INV
relationship: variable_of INV:0000036 ! Fruit Volume

[Term] 
id: INV:0000151
name: Fruit Volume - Volume of fruit calculation using minor axis of ellipse from Cut Side Up Image - mm^3
def: "Fruit is cut in half and imaged cut side up. Volume is calculated based on minor axis of the fitted ellipse (V=(Ï€d^3)/6)" []
namespace: INV
relationship: variable_of INV:0000036 ! Fruit Volume

[Term] 
id: INV:0000152
name: Fruit Water Activity - Aqualab 4TE Fruit Water Activity Measurement - Water activity
def: "Fruit water activity using the Aqualab 4TE meter." []
namespace: INV
relationship: variable_of INV:0000037 ! Fruit Water Activity

[Term] 
id: INV:0000153
name: Fruit Water Activity - WP4C Fruit Water Activity Measurement - Water activity
def: "Fruit water activity using the WP4C Dewpoint PotentiaMeter." []
namespace: INV
relationship: variable_of INV:0000037 ! Fruit Water Activity

[Term] 
id: INV:0000154
name: Fruit Water Loss - Fruit Water Loss Calculation - percentage
def: "Fruit water loss calculation. WatLoss = (Fresh Weight - Dry Weight)/(Fresh Weight)" []
namespace: INV
relationship: variable_of INV:0000038 ! Fruit Water Loss

[Term] 
id: INV:0000155
name: Fruit Water Potential - WP4C Fruit Water Potential Measurement - Megapascal
def: "Fruit water potential using the WP4C Dewpoint PotentiaMeter." []
namespace: INV
relationship: variable_of INV:0000039 ! Fruit Water Potential

[Term] 
id: INV:0000156
name: Graft Survival - Graft Survival Status - 0-1 Dead/Alive
def: "Date tree graft was evaluated for survival." []
namespace: INV
relationship: variable_of INV:0000040 ! Graft Survival

[Term] 
id: INV:0000157
name: Graft Survival Date - Graft Survival Date - YYYY-MM-DD
def: "Survival status of tree graft." []
namespace: INV
relationship: variable_of INV:0000041 ! Graft Survival Date

[Term] 
id: INV:0000158
name: Juice Percent - Calculation of Juice Percentage in Fruit - percentage
def: "Total Juice Weight divided by Total Fruit Weight for a Fruit Sample" []
namespace: INV
relationship: variable_of INV:0000042 ! Juice Percent

[Term] 
id: INV:0000159
name: Juice Weight - Juice Sample Weight Measurement - grams
def: "Juice weight of a fruit sample in grams." []
namespace: INV
relationship: variable_of INV:0000043 ! Juice Weight

[Term] 
id: INV:0000160
name: Juice Weight - Juice Sample Weight Measurement - kilograms
def: "Juice weight of a fruit sample in kilograms." []
namespace: INV
relationship: variable_of INV:0000043 ! Juice Weight

[Term] 
id: INV:0000161
name: Leaf Collection Date - Leaf Collection Date - YYYY-MM-DD
def: "Date leaf sample was collected." []
namespace: INV
relationship: variable_of INV:0000044 ! Leaf Collection Date

[Term] 
id: INV:0000162
name: Leaf Conductance - Leaf Conductance Measurement - mmol/(m²·s)
def: "Leaf conductance of sample using a leaf porometer" []
namespace: INV
relationship: variable_of INV:0000045 ! Leaf Conductance

[Term] 
id: INV:0000163
name: Leaf Relative Humidity - Leaf Relative Humidity Measurement - percentage
def: "Leaf relative humidity of sample using a leaf porometer" []
namespace: INV
relationship: variable_of INV:0000046 ! Leaf Relative Humidity

[Term] 
id: INV:0000164
name: Leaf Relative Water Content - Leaf Relative Water Content Calculation - percentage
def: "Relative water content calculation of a leaf sample. RWC = (fresh weight - dry weight)/(turgid weight - dry weight)" []
namespace: INV
relationship: variable_of INV:0000047 ! Leaf Relative Water Content

[Term] 
id: INV:0000165
name: Leaf Water Loss - Leaf Water Loss Calculation - percentage
def: "Leaf water loss calculation. WatLoss = (Fresh Weight - Dry Weight)/(Fresh Weight)" []
namespace: INV
relationship: variable_of INV:0000048 ! Leaf Water Loss

[Term] 
id: INV:0000166
name: Rootstock Trunk Diameter - Scion Diameter East to West Measurement - centimeters
def: "Measurement of scion diameter just below bud union from East to West in cm." []
namespace: INV
relationship: variable_of INV:0000049 ! Rootstock Trunk Diameter

[Term] 
id: INV:0000167
name: Rootstock Trunk Diameter - Scion Diameter East to West Measurement - inches
def: "Measurement of diameter just below bud union from East to West in inches." []
namespace: INV
relationship: variable_of INV:0000049 ! Rootstock Trunk Diameter

[Term] 
id: INV:0000168
name: Rootstock Trunk Diameter - Scion Diameter North to South Measurement - centimeters
def: "Measurement of scion diameter just below bud union from North to South in cm." []
namespace: INV
relationship: variable_of INV:0000049 ! Rootstock Trunk Diameter

[Term] 
id: INV:0000169
name: Rootstock Trunk Diameter - Scion Diameter North to South Measurement - inches
def: "Measurement of scion diameter just below bud union from North to South in inches." []
namespace: INV
relationship: variable_of INV:0000049 ! Rootstock Trunk Diameter

[Term] 
id: INV:0000170
name: Sampled Fruit Number - Sampled Fruit Count - count
def: "The number of fruit in a sample used for analysis" []
namespace: INV
relationship: variable_of INV:0000050 ! Sampled Fruit Number

[Term] 
id: INV:0000171
name: Scion Trunk Diameter - Scion Diameter East to West - centimeters
def: "Measurement of scion diameter just above bud union from East to West in cm." []
namespace: INV
relationship: variable_of INV:0000051 ! Scion Trunk Diameter

[Term] 
id: INV:0000172
name: Scion Trunk Diameter - Scion Diameter East to West Measurement - inches
def: "Measurement of scion diameter just above bud union from East to West in inches." []
namespace: INV
relationship: variable_of INV:0000051 ! Scion Trunk Diameter

[Term] 
id: INV:0000173
name: Scion Trunk Diameter - Scion Diameter North to South - centimeters
def: "Measurement of scion diameter just above bud union from North to South in cm." []
namespace: INV
relationship: variable_of INV:0000051 ! Scion Trunk Diameter

[Term] 
id: INV:0000174
name: Scion Trunk Diameter - Scion Diameter North to South Measurement - inches
def: "Measurement of scion diameter just above bud union from North to South in inches." []
namespace: INV
relationship: variable_of INV:0000051 ! Scion Trunk Diameter

[Term] 
id: INV:0000175
name: Seed Count - Seed Count - count
def: "Count of all seeds in a fruit sample." []
namespace: INV
relationship: variable_of INV:0000052 ! Seed Count

[Term] 
id: INV:0000176
name: Seed Water Loss - Seed Water Loss Calculation - percentage
def: "Seed water loss calculation. WatLoss = (Fresh Weight - Dry Weight)/(Fresh Weight)" []
namespace: INV
relationship: variable_of INV:0000053 ! Seed Water Loss

[Term] 
id: INV:0000177
name: Soil Moisture - Soil Moisture Measurement - 1-3 Soil Moisture Scale
def: "Estimation of soil moisture using a rating scale." []
namespace: INV
relationship: variable_of INV:0000054 ! Soil Moisture

[Term] 
id: INV:0000178
name: Soil Moisture - Soil Moisture Measurement - water fraction by volume
def: "Measurement of soil moisture using a soil moisture probe" []
namespace: INV
relationship: variable_of INV:0000054 ! Soil Moisture

[Term] 
id: INV:0000179
name: Total Soluble Solids - TSS Measurement - Degrees Brix
def: "Brix (total soluble solids) measurement in juice from fruit sample with refractometer." []
namespace: INV
relationship: variable_of INV:0000055 ! Total Soluble Solids

[Term] 
id: INV:0000180
name: Tree Yield - Count of Fruit on Tree using ML - count
def: "Count of Fruit on Tree using Machine Learning on Image of Tree" []
namespace: INV
relationship: variable_of INV:0000056 ! Tree Yield

[Term] 
id: INV:0000181
name: Tree Yield - Manual Count of Fruit on Tree - count
def: "Manual Count of Fruit on Tree" []
namespace: INV
relationship: variable_of INV:0000056 ! Tree Yield

[Term] 
id: INV:0000182
name: Tree Yield - Weight of All Fruit Harvested - pounds
def: "Weight of all Fruit on Tree Harvested for Yield Estimation in kilograms." []
namespace: INV
relationship: variable_of INV:0000056 ! Tree Yield

[Term] 
id: INV:0000183
name: Turgid Leaf Weight - Turgid Leaf Tissue Weight Measurement - grams
def: "Leaf sample weight in grams after soaked in distilled water for 3 hours in the dark at room temp." []
namespace: INV
relationship: variable_of INV:0000057 ! Turgid Leaf Weight

[Term] 
id: INV:0000184
name: Wet Soil Weight - Wet Soil Weight Measurement - grams
def: "Direct measurement of the weight of a soil sample when freshly collected." []
namespace: INV
relationship: variable_of INV:0000058 ! Wet Soil Weight

